Source/Dafny/DafnyPrelude.bpl
@@ -8,7 +8,7 @@
 // SPDX-License-Identifier: MIT
 
 const $$Language$Dafny: bool;  // To be recognizable to the ModelViewer as
-axiom $$Language$Dafny;        // coming from a Dafny program.
+axiom {:root} $$Language$Dafny;        // coming from a Dafny program.
 
 // ---------------------------------------------------------------
 // -- Types ------------------------------------------------------
@@ -17,120 +17,129 @@ axiom $$Language$Dafny;        // coming from a Dafny program.
 type Ty;
 type Bv0 = int;
 
-const unique TBool : Ty;
-const unique TChar : Ty;
-const unique TInt  : Ty;
-const unique TReal : Ty;
-const unique TORDINAL  : Ty;
-function TBitvector(int) : Ty;
-function TSet(Ty)      : Ty;
-function TISet(Ty)     : Ty;
-function TMultiSet(Ty) : Ty;
-function TSeq(Ty)      : Ty;
-function TMap(Ty, Ty)  : Ty;
-function TIMap(Ty, Ty) : Ty;
+const unique TBool : Ty uses {
+  axiom Tag(TBool) == TagBool;
+}
+const unique TChar : Ty uses {
+  axiom Tag(TChar) == TagChar;
+}
+const unique TInt  : Ty uses {
+  axiom Tag(TInt) == TagInt;
+}
+const unique TReal : Ty uses {
+  axiom Tag(TReal) == TagReal;
+}
+const unique TORDINAL  : Ty uses {
+  axiom Tag(TORDINAL) == TagORDINAL;
+}
+// See for which axioms we can make use of the trigger to determine the connection.
+function TBitvector(int) : Ty uses {
+  axiom (forall w: int :: { TBitvector(w) } Inv0_TBitvector(TBitvector(w)) == w);
+}
+function TSet(Ty)      : Ty uses {
+  axiom (forall t: Ty :: { TSet(t) } Inv0_TSet(TSet(t)) == t);
+  axiom (forall t: Ty    :: { TSet(t) }      Tag(TSet(t))      == TagSet);
+}
+function TISet(Ty)     : Ty uses {
+  axiom (forall t: Ty :: { TISet(t) } Inv0_TISet(TISet(t)) == t);
+  axiom (forall t: Ty    :: { TISet(t) }     Tag(TISet(t))     == TagISet);
+}
+function TMultiSet(Ty) : Ty uses {
+  axiom (forall t: Ty :: { TMultiSet(t) } Inv0_TMultiSet(TMultiSet(t)) == t);
+  axiom (forall t: Ty    :: { TMultiSet(t) } Tag(TMultiSet(t)) == TagMultiSet);
+}
+function TSeq(Ty)      : Ty uses {
+  axiom (forall t: Ty :: { TSeq(t) } Inv0_TSeq(TSeq(t)) == t);
+  axiom (forall t: Ty    :: { TSeq(t) }      Tag(TSeq(t))      == TagSeq);
+}
+function TMap(Ty, Ty)  : Ty uses {
+  axiom (forall t, u: Ty :: { TMap(t,u) } Inv0_TMap(TMap(t,u)) == t);
+  axiom (forall t, u: Ty :: { TMap(t,u) } Inv1_TMap(TMap(t,u)) == u);
+  axiom (forall t, u: Ty :: { TMap(t,u) }    Tag(TMap(t,u))    == TagMap);
+}
+function TIMap(Ty, Ty) : Ty uses {
+  axiom (forall t, u: Ty :: { TIMap(t,u) } Inv0_TIMap(TIMap(t,u)) == t);
+  axiom (forall t, u: Ty :: { TIMap(t,u) } Inv1_TIMap(TIMap(t,u)) == u);
+  axiom (forall t, u: Ty :: { TIMap(t,u) }   Tag(TIMap(t,u))   == TagIMap);
+}
 
 function Inv0_TBitvector(Ty) : int;
-axiom (forall w: int :: { TBitvector(w) } Inv0_TBitvector(TBitvector(w)) == w);
 function Inv0_TSet(Ty) : Ty;
-axiom (forall t: Ty :: { TSet(t) } Inv0_TSet(TSet(t)) == t);
 function Inv0_TISet(Ty) : Ty;
-axiom (forall t: Ty :: { TISet(t) } Inv0_TISet(TISet(t)) == t);
 function Inv0_TSeq(Ty) : Ty;
-axiom (forall t: Ty :: { TSeq(t) } Inv0_TSeq(TSeq(t)) == t);
 function Inv0_TMultiSet(Ty) : Ty;
-axiom (forall t: Ty :: { TMultiSet(t) } Inv0_TMultiSet(TMultiSet(t)) == t);
 function Inv0_TMap(Ty) : Ty;
 function Inv1_TMap(Ty) : Ty;
-axiom (forall t, u: Ty :: { TMap(t,u) } Inv0_TMap(TMap(t,u)) == t);
-axiom (forall t, u: Ty :: { TMap(t,u) } Inv1_TMap(TMap(t,u)) == u);
 function Inv0_TIMap(Ty) : Ty;
 function Inv1_TIMap(Ty) : Ty;
-axiom (forall t, u: Ty :: { TIMap(t,u) } Inv0_TIMap(TIMap(t,u)) == t);
-axiom (forall t, u: Ty :: { TIMap(t,u) } Inv1_TIMap(TIMap(t,u)) == u);
 
 // -- Classes and Datatypes --
 
 // -- Type Tags --
 type TyTag;
-function {:exclude_dep} Tag(Ty) : TyTag;
+function Tag(Ty) : TyTag;
 
-const unique TagBool     : TyTag uses {
-    axiom Tag(TBool) == TagBool;
-}
-const unique TagChar     : TyTag uses {
-    axiom Tag(TChar) == TagChar;
-}
-const unique TagInt      : TyTag uses {
-    axiom Tag(TInt) == TagInt;
-}
-const unique TagReal     : TyTag uses {
-    axiom Tag(TReal) == TagReal;
-}
-const unique TagORDINAL  : TyTag uses {
-    axiom Tag(TORDINAL) == TagORDINAL;
-}
-const unique TagSet      : TyTag uses {
-    axiom (forall t: Ty    :: { TSet(t) }      Tag(TSet(t))      == TagSet);
-}
-const unique TagISet     : TyTag uses {
-    axiom (forall t: Ty    :: { TISet(t) }     Tag(TISet(t))     == TagISet);
-}
-const unique TagMultiSet : TyTag uses {
-    axiom (forall t: Ty    :: { TMultiSet(t) } Tag(TMultiSet(t)) == TagMultiSet);
-}
-const unique TagSeq      : TyTag uses {
-    axiom (forall t: Ty    :: { TSeq(t) }      Tag(TSeq(t))      == TagSeq);
-}
-const unique TagMap      : TyTag uses {
-    axiom (forall t, u: Ty :: { TMap(t,u) }    Tag(TMap(t,u))    == TagMap);
-}
-const unique TagIMap     : TyTag uses {    
-    axiom (forall t, u: Ty :: { TIMap(t,u) }   Tag(TIMap(t,u))   == TagIMap);
-}
+const unique TagBool     : TyTag;
+const unique TagChar     : TyTag;
+const unique TagInt      : TyTag;
+const unique TagReal     : TyTag;
+const unique TagORDINAL  : TyTag;
+const unique TagSet      : TyTag;
+const unique TagISet     : TyTag;
+const unique TagMultiSet : TyTag;
+const unique TagSeq      : TyTag;
+const unique TagMap      : TyTag;
+const unique TagIMap     : TyTag;
 const unique TagClass    : TyTag;
 
 type TyTagFamily;
-function {:exclude_dep} TagFamily(Ty): TyTagFamily;
+function TagFamily(Ty): TyTagFamily;
 
 // ---------------------------------------------------------------
 // -- Literals ---------------------------------------------------
 // ---------------------------------------------------------------
-function {:identity} {:exclude_dep} Lit<T>(x: T): T { x } uses {
+function {:identity} Lit<T>(x: T): T { x } uses {
   axiom (forall<T> x: T :: { $Box(Lit(x)) } $Box(Lit(x)) == Lit($Box(x)) );
 }
 
 // Specialize Lit to concrete types.
 // These aren't logically required, but on some examples improve
 // verification speed
-function {:identity} LitInt(x: int): int { x }
-axiom (forall x: int :: { $Box(LitInt(x)) } $Box(LitInt(x)) == Lit($Box(x)) );
-function {:identity} LitReal(x: real): real { x }
-axiom (forall x: real :: { $Box(LitReal(x)) } $Box(LitReal(x)) == Lit($Box(x)) );
+function {:identity} LitInt(x: int): int { x } uses {
+  axiom (forall x: int :: { $Box(LitInt(x)) } $Box(LitInt(x)) == Lit($Box(x)) );
+}
+function {:identity} LitReal(x: real): real { x } uses {
+  axiom (forall x: real :: { $Box(LitReal(x)) } $Box(LitReal(x)) == Lit($Box(x)) );
+}
 
 // ---------------------------------------------------------------
 // -- Characters -------------------------------------------------
 // ---------------------------------------------------------------
 
 type char;
-function char#FromInt(int): char;
-function char#ToInt(char): int;  // inverse of char#FromInt
-axiom (forall ch: char ::
-  { char#ToInt(ch) }
-  char#FromInt(char#ToInt(ch)) == ch &&
-  0 <= char#ToInt(ch) && char#ToInt(ch) < 65536);
-axiom (forall n: int ::
-  { char#FromInt(n) }
-  0 <= n && n < 65536 ==> char#ToInt(char#FromInt(n)) == n);
+function char#FromInt(int): char uses {
+  axiom (forall n: int ::
+    { char#FromInt(n) }
+    0 <= n && n < 65536 ==> char#ToInt(char#FromInt(n)) == n);
+}
 
-function char#Plus(char, char): char;
-function char#Minus(char, char): char;
-axiom (forall a: char, b: char ::
-  { char#Plus(a, b) }
-  char#Plus(a, b) == char#FromInt(char#ToInt(a) + char#ToInt(b)));
-axiom (forall a: char, b: char ::
-  { char#Minus(a, b) }
-  char#Minus(a, b) == char#FromInt(char#ToInt(a) - char#ToInt(b)));
+function char#ToInt(char): int uses {
+  axiom (forall ch: char ::
+    { char#ToInt(ch) }
+    char#FromInt(char#ToInt(ch)) == ch &&
+    0 <= char#ToInt(ch) && char#ToInt(ch) < 65536);
+}  
+
+function char#Plus(char, char): char uses {
+  axiom (forall a: char, b: char ::
+    { char#Plus(a, b) }
+    char#Plus(a, b) == char#FromInt(char#ToInt(a) + char#ToInt(b)));
+}
+function char#Minus(char, char): char uses {
+  axiom (forall a: char, b: char ::
+    { char#Minus(a, b) }
+    char#Minus(a, b) == char#FromInt(char#ToInt(a) - char#ToInt(b)));
+}
 
 // ---------------------------------------------------------------
 // -- References -------------------------------------------------
@@ -146,53 +155,58 @@ const null: ref;
 type Box;
 const $ArbitraryBoxValue: Box;
 
-function $Box<T>(T): Box;
+function $Box<T>(T): Box uses {
+  axiom (forall<T> x : T :: { $Box(x) } $Unbox($Box(x)) == x);
+}
 function $Unbox<T>(Box): T;
 
-axiom (forall<T> x : T :: { $Box(x) } $Unbox($Box(x)) == x);
+// Corresponding entries for boxes...
+// This could probably be solved by having Box also inhabit Ty
+function $IsBox<T>(T,Ty): bool;
+function $IsAllocBox<T>(T,Ty,Heap): bool;
 
-axiom (forall bx : Box ::
+axiom {:root} (forall bx : Box ::
     { $IsBox(bx, TInt) }
     ( $IsBox(bx, TInt) ==> $Box($Unbox(bx) : int) == bx && $Is($Unbox(bx) : int, TInt)));
-axiom (forall bx : Box ::
+axiom {:root} (forall bx : Box ::
     { $IsBox(bx, TReal) }
     ( $IsBox(bx, TReal) ==> $Box($Unbox(bx) : real) == bx && $Is($Unbox(bx) : real, TReal)));
-axiom (forall bx : Box ::
+axiom {:root} (forall bx : Box ::
     { $IsBox(bx, TBool) }
     ( $IsBox(bx, TBool) ==> $Box($Unbox(bx) : bool) == bx && $Is($Unbox(bx) : bool, TBool)));
-axiom (forall bx : Box ::
+axiom {:root} (forall bx : Box ::
     { $IsBox(bx, TChar) }
     ( $IsBox(bx, TChar) ==> $Box($Unbox(bx) : char) == bx && $Is($Unbox(bx) : char, TChar)));
 
 // Since each bitvector type is a separate type in Boogie, the Box/Unbox axioms for bitvectors are
 // generated programmatically. Except, Bv0 is given here.
-axiom (forall bx : Box ::
+axiom {:root} (forall bx : Box ::
     { $IsBox(bx, TBitvector(0)) }
     ( $IsBox(bx, TBitvector(0)) ==> $Box($Unbox(bx) : Bv0) == bx && $Is($Unbox(bx) : Set Box, TBitvector(0))));
 
-axiom (forall bx : Box, t : Ty ::
+axiom {:root} (forall bx : Box, t : Ty ::
     { $IsBox(bx, TSet(t)) }
     ( $IsBox(bx, TSet(t)) ==> $Box($Unbox(bx) : Set Box) == bx && $Is($Unbox(bx) : Set Box, TSet(t))));
-axiom (forall bx : Box, t : Ty ::
+axiom {:root} (forall bx : Box, t : Ty ::
     { $IsBox(bx, TISet(t)) }
     ( $IsBox(bx, TISet(t)) ==> $Box($Unbox(bx) : ISet Box) == bx && $Is($Unbox(bx) : ISet Box, TISet(t))));
-axiom (forall bx : Box, t : Ty ::
+axiom {:root} (forall bx : Box, t : Ty ::
     { $IsBox(bx, TMultiSet(t)) }
     ( $IsBox(bx, TMultiSet(t)) ==> $Box($Unbox(bx) : MultiSet Box) == bx && $Is($Unbox(bx) : MultiSet Box, TMultiSet(t))));
-axiom (forall bx : Box, t : Ty ::
+axiom {:root} (forall bx : Box, t : Ty ::
     { $IsBox(bx, TSeq(t)) }
     ( $IsBox(bx, TSeq(t)) ==> $Box($Unbox(bx) : Seq Box) == bx && $Is($Unbox(bx) : Seq Box, TSeq(t))));
-axiom (forall bx : Box, s : Ty, t : Ty ::
+axiom {:root} (forall bx : Box, s : Ty, t : Ty ::
     { $IsBox(bx, TMap(s, t)) }
     ( $IsBox(bx, TMap(s, t)) ==> $Box($Unbox(bx) : Map Box Box) == bx && $Is($Unbox(bx) : Map Box Box, TMap(s, t))));
-axiom (forall bx : Box, s : Ty, t : Ty ::
+axiom {:root} (forall bx : Box, s : Ty, t : Ty ::
     { $IsBox(bx, TIMap(s, t)) }
     ( $IsBox(bx, TIMap(s, t)) ==> $Box($Unbox(bx) : IMap Box Box) == bx && $Is($Unbox(bx) : IMap Box Box, TIMap(s, t))));
 
-axiom (forall<T> v : T, t : Ty ::
+axiom {:root} (forall<T> v : T, t : Ty ::
     { $IsBox($Box(v), t) }
     ( $IsBox($Box(v), t) <==> $Is(v,t) ));
-axiom (forall<T> v : T, t : Ty, h : Heap ::
+axiom {:root} (forall<T> v : T, t : Ty, h : Heap ::
     { $IsAllocBox($Box(v), t, h) }
     ( $IsAllocBox($Box(v), t, h) <==> $IsAlloc(v,t,h) ));
 
@@ -202,7 +216,7 @@ axiom (forall<T> v : T, t : Ty, h : Heap ::
 
 // Type-argument to $Is is the /representation type/,
 // the second value argument to $Is is the actual type.
-function {:exclude_dep} $Is<T>(T,Ty): bool uses {           // no heap for now
+function $Is<T>(T,Ty): bool uses {           // no heap for now
     axiom(forall v : int  :: { $Is(v,TInt) }  $Is(v,TInt));
     axiom(forall v : real :: { $Is(v,TReal) } $Is(v,TReal));
     axiom(forall v : bool :: { $Is(v,TBool) } $Is(v,TBool));
@@ -263,7 +277,7 @@ function {:exclude_dep} $Is<T>(T,Ty): bool uses {           // no heap for now
         $Is(IMap#Values(v), TISet(t1)) &&
         $Is(IMap#Items(v), TISet(Tclass._System.Tuple2(t0, t1))));
 }
-function {:exclude_dep}  $IsAlloc<T>(T,Ty,Heap): bool uses {
+function  $IsAlloc<T>(T,Ty,Heap): bool uses {
     axiom(forall h : Heap, v : int  :: { $IsAlloc(v,TInt,h) }  $IsAlloc(v,TInt,h));
     axiom(forall h : Heap, v : real :: { $IsAlloc(v,TReal,h) } $IsAlloc(v,TReal,h));
     axiom(forall h : Heap, v : bool :: { $IsAlloc(v,TBool,h) } $IsAlloc(v,TBool,h));
@@ -309,11 +323,6 @@ function {:exclude_dep}  $IsAlloc<T>(T,Ty,Heap): bool uses {
             $IsAllocBox(bx, t0, h)));
 }
 
-// Corresponding entries for boxes...
-// This could probably be solved by having Box also inhabit Ty
-function $IsBox<T>(T,Ty): bool;
-function $IsAllocBox<T>(T,Ty,Heap): bool;
-
 // ---------------------------------------------------------------
 // -- Encoding of type names -------------------------------------
 // ---------------------------------------------------------------
@@ -334,7 +343,7 @@ function TypeTuple(a: ClassName, b: ClassName): ClassName;
 function TypeTupleCar(ClassName): ClassName;
 function TypeTupleCdr(ClassName): ClassName;
 // TypeTuple is injective in both arguments:
-axiom (forall a: ClassName, b: ClassName :: { TypeTuple(a,b) }
+axiom {:root} (forall a: ClassName, b: ClassName :: { TypeTuple(a,b) }
   TypeTupleCar(TypeTuple(a,b)) == a &&
   TypeTupleCdr(TypeTuple(a,b)) == b);
 
@@ -343,9 +352,9 @@ axiom (forall a: ClassName, b: ClassName :: { TypeTuple(a,b) }
 type HandleType;
 
 function SetRef_to_SetBox(s: [ref]bool): Set Box;
-axiom (forall s: [ref]bool, bx: Box :: { SetRef_to_SetBox(s)[bx] }
+axiom {:root} (forall s: [ref]bool, bx: Box :: { SetRef_to_SetBox(s)[bx] }
   SetRef_to_SetBox(s)[bx] == s[$Unbox(bx): ref]);
-axiom (forall s: [ref]bool :: { SetRef_to_SetBox(s) }
+axiom {:root} (forall s: [ref]bool :: { SetRef_to_SetBox(s) }
   $Is(SetRef_to_SetBox(s), TSet(Tclass._System.object?())));
 
 // Functions ApplyN, RequiresN, and ReadsN are generated on demand by the translator,
@@ -359,12 +368,12 @@ function Apply1(Ty, Ty, Heap, HandleType, Box): Box;
 type DatatypeType;
 
 type DtCtorId;
-function {:exclude_dep} DatatypeCtorId(DatatypeType): DtCtorId;
+function DatatypeCtorId(DatatypeType): DtCtorId;
 
 function DtRank(DatatypeType): int;
 function BoxRank(Box): int;
 
-axiom (forall d: DatatypeType :: {BoxRank($Box(d))} BoxRank($Box(d)) == DtRank(d));
+axiom {:root} (forall d: DatatypeType :: {BoxRank($Box(d))} BoxRank($Box(d)) == DtRank(d));
 
 // ---------------------------------------------------------------
 // -- Big Ordinals -----------------------------------------------
@@ -379,78 +388,78 @@ type ORDINAL = Box;  // :| There are more big ordinals than boxes
 // That is, if the ordinal is \lambda+n, then ORD#Offset returns n.
 function ORD#IsNat(ORDINAL): bool;
 function ORD#Offset(ORDINAL): int;
-axiom (forall o:ORDINAL :: { ORD#Offset(o) } 0 <= ORD#Offset(o));
+axiom {:root} (forall o:ORDINAL :: { ORD#Offset(o) } 0 <= ORD#Offset(o));
 
 function {:inline} ORD#IsLimit(o: ORDINAL): bool { ORD#Offset(o) == 0 }
 function {:inline} ORD#IsSucc(o: ORDINAL): bool { 0 < ORD#Offset(o) }
 
 function ORD#FromNat(int): ORDINAL;
-axiom (forall n:int :: { ORD#FromNat(n) }
+axiom {:root} (forall n:int :: { ORD#FromNat(n) }
   0 <= n ==> ORD#IsNat(ORD#FromNat(n)) && ORD#Offset(ORD#FromNat(n)) == n);
-axiom (forall o:ORDINAL :: { ORD#Offset(o) } { ORD#IsNat(o) }
+axiom {:root} (forall o:ORDINAL :: { ORD#Offset(o) } { ORD#IsNat(o) }
   ORD#IsNat(o) ==> o == ORD#FromNat(ORD#Offset(o)));
 
 function ORD#Less(ORDINAL, ORDINAL): bool;
-axiom (forall o,p: ORDINAL :: { ORD#Less(o,p) }
+axiom {:root} (forall o,p: ORDINAL :: { ORD#Less(o,p) }
   (ORD#Less(o,p) ==> o != p) &&  // irreflexivity
   (ORD#IsNat(o) && !ORD#IsNat(p) ==> ORD#Less(o,p)) &&
   (ORD#IsNat(o) && ORD#IsNat(p) ==> ORD#Less(o,p) == (ORD#Offset(o) < ORD#Offset(p))) &&
   (ORD#Less(o,p) && ORD#IsNat(p) ==> ORD#IsNat(o)));
 // ORD#Less is trichotomous:
-axiom (forall o,p: ORDINAL :: { ORD#Less(o,p), ORD#Less(p,o) }
+axiom {:root} (forall o,p: ORDINAL :: { ORD#Less(o,p), ORD#Less(p,o) }
   ORD#Less(o,p) || o == p || ORD#Less(p,o));
 // ORD#Less is transitive:
-axiom (forall o,p,r: ORDINAL ::
+axiom {:root} (forall o,p,r: ORDINAL ::
   { ORD#Less(o,p), ORD#Less(p,r) }
   { ORD#Less(o,p), ORD#Less(o,r) }
   ORD#Less(o,p) && ORD#Less(p,r) ==> ORD#Less(o,r));
 
 // ORD#LessThanLimit is a synonym of ORD#Less, introduced for more selected triggering
 function ORD#LessThanLimit(ORDINAL, ORDINAL): bool;
-axiom (forall o,p: ORDINAL :: { ORD#LessThanLimit(o, p) }
+axiom {:root} (forall o,p: ORDINAL :: { ORD#LessThanLimit(o, p) }
   ORD#LessThanLimit(o, p) == ORD#Less(o, p));
 
 function ORD#Plus(ORDINAL, ORDINAL): ORDINAL;
-axiom (forall o,p: ORDINAL :: { ORD#Plus(o,p) }
+axiom {:root} (forall o,p: ORDINAL :: { ORD#Plus(o,p) }
   (ORD#IsNat(ORD#Plus(o,p)) ==> ORD#IsNat(o) && ORD#IsNat(p)) &&
   (ORD#IsNat(p) ==>
     ORD#IsNat(ORD#Plus(o,p)) == ORD#IsNat(o) &&
     ORD#Offset(ORD#Plus(o,p)) == ORD#Offset(o) + ORD#Offset(p)));
-axiom (forall o,p: ORDINAL :: { ORD#Plus(o,p) }
+axiom {:root} (forall o,p: ORDINAL :: { ORD#Plus(o,p) }
   (o == ORD#Plus(o, p) || ORD#Less(o, ORD#Plus(o, p))) &&
   (p == ORD#Plus(o, p) || ORD#Less(p, ORD#Plus(o, p))));
-axiom (forall o,p: ORDINAL :: { ORD#Plus(o,p) }
+axiom {:root} (forall o,p: ORDINAL :: { ORD#Plus(o,p) }
   (o == ORD#FromNat(0) ==> ORD#Plus(o, p) == p) &&
   (p == ORD#FromNat(0) ==> ORD#Plus(o, p) == o));
 
 function ORD#Minus(ORDINAL, ORDINAL): ORDINAL;
-axiom (forall o,p: ORDINAL :: { ORD#Minus(o,p) }
+axiom {:root} (forall o,p: ORDINAL :: { ORD#Minus(o,p) }
   ORD#IsNat(p) && ORD#Offset(p) <= ORD#Offset(o) ==>
     ORD#IsNat(ORD#Minus(o,p)) == ORD#IsNat(o) &&
     ORD#Offset(ORD#Minus(o,p)) == ORD#Offset(o) - ORD#Offset(p));
-axiom (forall o,p: ORDINAL :: { ORD#Minus(o,p) }
+axiom {:root} (forall o,p: ORDINAL :: { ORD#Minus(o,p) }
   ORD#IsNat(p) && ORD#Offset(p) <= ORD#Offset(o) ==>
     (p == ORD#FromNat(0) && ORD#Minus(o, p) == o) ||
     (p != ORD#FromNat(0) && ORD#Less(ORD#Minus(o, p), o)));
 
 // o+m+n == o+(m+n)
-axiom (forall o: ORDINAL, m,n: int ::
+axiom {:root} (forall o: ORDINAL, m,n: int ::
   { ORD#Plus(ORD#Plus(o, ORD#FromNat(m)), ORD#FromNat(n)) }
   0 <= m && 0 <= n ==>
   ORD#Plus(ORD#Plus(o, ORD#FromNat(m)), ORD#FromNat(n)) == ORD#Plus(o, ORD#FromNat(m+n)));
 // o-m-n == o+(m+n)
-axiom (forall o: ORDINAL, m,n: int ::
+axiom {:root} (forall o: ORDINAL, m,n: int ::
   { ORD#Minus(ORD#Minus(o, ORD#FromNat(m)), ORD#FromNat(n)) }
   0 <= m && 0 <= n && m+n <= ORD#Offset(o) ==>
   ORD#Minus(ORD#Minus(o, ORD#FromNat(m)), ORD#FromNat(n)) == ORD#Minus(o, ORD#FromNat(m+n)));
 // o+m-n == EITHER o+(m-n) OR o-(n-m)
-axiom (forall o: ORDINAL, m,n: int ::
+axiom {:root} (forall o: ORDINAL, m,n: int ::
   { ORD#Minus(ORD#Plus(o, ORD#FromNat(m)), ORD#FromNat(n)) }
   0 <= m && 0 <= n && n <= ORD#Offset(o) + m ==>
     (0 <= m - n ==> ORD#Minus(ORD#Plus(o, ORD#FromNat(m)), ORD#FromNat(n)) == ORD#Plus(o, ORD#FromNat(m-n))) &&
     (m - n <= 0 ==> ORD#Minus(ORD#Plus(o, ORD#FromNat(m)), ORD#FromNat(n)) == ORD#Minus(o, ORD#FromNat(n-m))));
 // o-m+n == EITHER o-(m-n) OR o+(n-m)
-axiom (forall o: ORDINAL, m,n: int ::
+axiom {:root} (forall o: ORDINAL, m,n: int ::
   { ORD#Plus(ORD#Minus(o, ORD#FromNat(m)), ORD#FromNat(n)) }
   0 <= m && 0 <= n && n <= ORD#Offset(o) + m ==>
     (0 <= m - n ==> ORD#Plus(ORD#Minus(o, ORD#FromNat(m)), ORD#FromNat(n)) == ORD#Minus(o, ORD#FromNat(m-n))) &&
@@ -462,7 +471,7 @@ axiom (forall o: ORDINAL, m,n: int ::
 
 // used to make sure function axioms are not used while their consistency is being checked
 const $ModuleContextHeight: int;
-const {:exclude_dep} $FunctionContextHeight: int;
+const $FunctionContextHeight: int;
 
 // ---------------------------------------------------------------
 // -- Layers of function encodings -------------------------------
@@ -474,8 +483,8 @@ function $LS(LayerType): LayerType;
 function AsFuelBottom(LayerType) : LayerType;
 
 function AtLayer<A>([LayerType]A, LayerType): A;
-axiom (forall<A> f : [LayerType]A, ly : LayerType :: { AtLayer(f,ly) } AtLayer(f,ly) == f[ly]);
-axiom (forall<A> f : [LayerType]A, ly : LayerType :: { AtLayer(f,$LS(ly)) } AtLayer(f,$LS(ly)) == AtLayer(f,ly));
+axiom {:root} (forall<A> f : [LayerType]A, ly : LayerType :: { AtLayer(f,ly) } AtLayer(f,ly) == f[ly]);
+axiom {:root} (forall<A> f : [LayerType]A, ly : LayerType :: { AtLayer(f,$LS(ly)) } AtLayer(f,$LS(ly)) == AtLayer(f,ly));
 
 // ---------------------------------------------------------------
 // -- Fields -----------------------------------------------------
@@ -483,18 +492,18 @@ axiom (forall<A> f : [LayerType]A, ly : LayerType :: { AtLayer(f,$LS(ly)) } AtLa
 
 type Field alpha;
 
-function {:exclude_dep} FDim<T>(Field T): int;
+function FDim<T>(Field T): int;
 
 function IndexField(int): Field Box;
-axiom (forall i: int :: { IndexField(i) } FDim(IndexField(i)) == 1);
+axiom {:root} (forall i: int :: { IndexField(i) } FDim(IndexField(i)) == 1);
 function IndexField_Inverse<T>(Field T): int;
-axiom (forall i: int :: { IndexField(i) } IndexField_Inverse(IndexField(i)) == i);
+axiom {:root} (forall i: int :: { IndexField(i) } IndexField_Inverse(IndexField(i)) == i);
 
 function MultiIndexField(Field Box, int): Field Box;
-axiom (forall f: Field Box, i: int :: { MultiIndexField(f,i) } FDim(MultiIndexField(f,i)) == FDim(f) + 1);
+axiom {:root} (forall f: Field Box, i: int :: { MultiIndexField(f,i) } FDim(MultiIndexField(f,i)) == FDim(f) + 1);
 function MultiIndexField_Inverse0<T>(Field T): Field T;
 function MultiIndexField_Inverse1<T>(Field T): int;
-axiom (forall f: Field Box, i: int :: { MultiIndexField(f,i) }
+axiom {:root} (forall f: Field Box, i: int :: { MultiIndexField(f,i) }
   MultiIndexField_Inverse0(MultiIndexField(f,i)) == f &&
   MultiIndexField_Inverse1(MultiIndexField(f,i)) == i);
 
@@ -503,12 +512,18 @@ function DeclType<T>(Field T): ClassName;
 type NameFamily;
 function DeclName<T>(Field T): NameFamily;
 function FieldOfDecl<alpha>(ClassName, NameFamily): Field alpha;
-axiom (forall<T> cl : ClassName, nm: NameFamily ::
+axiom {:root} (forall<T> cl : ClassName, nm: NameFamily ::
    {FieldOfDecl(cl, nm): Field T}
    DeclType(FieldOfDecl(cl, nm): Field T) == cl && DeclName(FieldOfDecl(cl, nm): Field T) == nm);
 
-function {:exclude_dep} $IsGhostField<T>(Field T): bool uses {
-  axiom !$IsGhostField(alloc); // treat as non-ghost field, because it cannot be changed by ghost code
+function $IsGhostField<T>(Field T): bool uses {
+   axiom $IsGhostField(alloc); // treat as ghost field, since it is allowed to be changed by ghost code
+  
+   axiom (forall h: Heap, k: Heap :: { $HeapSuccGhost(h,k) }
+      $HeapSuccGhost(h,k) ==>
+        $HeapSucc(h,k) &&
+        (forall<alpha> o: ref, f: Field alpha :: { read(k, o, f) }
+          !$IsGhostField(f) ==> read(h, o, f) == read(k, o, f)));
 }
 
 // ---------------------------------------------------------------
@@ -518,10 +533,10 @@ function {:exclude_dep} $IsGhostField<T>(Field T): bool uses {
 
 // $IsAlloc and $IsAllocBox are monotonic
 
-axiom(forall<T> h, k : Heap, v : T, t : Ty ::
+axiom {:root} (forall<T> h, k : Heap, v : T, t : Ty ::
   { $HeapSucc(h, k), $IsAlloc(v, t, h) }
   $HeapSucc(h, k) ==> $IsAlloc(v, t, h) ==> $IsAlloc(v, t, k));
-axiom(forall h, k : Heap, bx : Box, t : Ty ::
+axiom {:root} (forall h, k : Heap, bx : Box, t : Ty ::
   { $HeapSucc(h, k), $IsAllocBox(bx, t, h) }
   $HeapSucc(h, k) ==> $IsAllocBox(bx, t, h) ==> $IsAllocBox(bx, t, k));
 
@@ -529,7 +544,7 @@ axiom(forall h, k : Heap, bx : Box, t : Ty ::
 
 const unique alloc: Field bool;
 const unique allocName: NameFamily;
-axiom FDim(alloc) == 0 &&
+axiom {:root} FDim(alloc) == 0 &&
   DeclName(alloc) == allocName;
 
 // ---------------------------------------------------------------
@@ -537,7 +552,7 @@ axiom FDim(alloc) == 0 &&
 // ---------------------------------------------------------------
 
 function _System.array.Length(a: ref): int;
-axiom (forall o: ref :: 0 <= _System.array.Length(o));
+axiom {:root} (forall o: ref :: 0 <= _System.array.Length(o));
 
 // ---------------------------------------------------------------
 // -- Reals ------------------------------------------------------
@@ -545,7 +560,7 @@ axiom (forall o: ref :: 0 <= _System.array.Length(o));
 
 function Int(x: real): int { int(x) }
 function Real(x: int): real { real(x) }
-axiom (forall i: int :: { Int(Real(i)) } Int(Real(i)) == i);
+axiom {:root} (forall i: int :: { Int(Real(i)) } Int(Real(i)) == i);
 
 function {:inline} _System.real.Floor(x: real): int { Int(x) }
 
@@ -564,23 +579,18 @@ var $Heap: Heap where $IsGoodHeap($Heap) && $IsHeapAnchor($Heap);
 // but the expression generated is really one that is (at least in a correct program)
 // independent of the heap.
 const $OneHeap: Heap;
-axiom $IsGoodHeap($OneHeap);
+axiom {:root} $IsGoodHeap($OneHeap);
 
 function $HeapSucc(Heap, Heap): bool;
-axiom (forall<alpha> h: Heap, r: ref, f: Field alpha, x: alpha :: { update(h, r, f, x) }
+axiom {:root} (forall<alpha> h: Heap, r: ref, f: Field alpha, x: alpha :: { update(h, r, f, x) }
   $IsGoodHeap(update(h, r, f, x)) ==>
   $HeapSucc(h, update(h, r, f, x)));
-axiom (forall a,b,c: Heap :: { $HeapSucc(a,b), $HeapSucc(b,c) }
+axiom {:root} (forall a,b,c: Heap :: { $HeapSucc(a,b), $HeapSucc(b,c) }
   a != c ==> $HeapSucc(a,b) && $HeapSucc(b,c) ==> $HeapSucc(a,c));
-axiom (forall h: Heap, k: Heap :: { $HeapSucc(h,k) }
+axiom {:root} (forall h: Heap, k: Heap :: { $HeapSucc(h,k) }
   $HeapSucc(h,k) ==> (forall o: ref :: { read(k, o, alloc) } read(h, o, alloc) ==> read(k, o, alloc)));
 
 function $HeapSuccGhost(Heap, Heap): bool;
-axiom (forall h: Heap, k: Heap :: { $HeapSuccGhost(h,k) }
-  $HeapSuccGhost(h,k) ==>
-    $HeapSucc(h,k) &&
-    (forall<alpha> o: ref, f: Field alpha :: { read(k, o, f) }
-      !$IsGhostField(f) ==> read(h, o, f) == read(k, o, f)));
 
 // ---------------------------------------------------------------
 // -- Non-determinism --------------------------------------------
@@ -637,11 +647,11 @@ procedure $IterCollectNewObjects(prevHeap: Heap, newHeap: Heap, this: ref, NW: F
 type Set T = [T]bool;
 
 function Set#Card<T>(Set T): int;
-axiom (forall<T> s: Set T :: { Set#Card(s) } 0 <= Set#Card(s));
+axiom {:root} (forall<T> s: Set T :: { Set#Card(s) } 0 <= Set#Card(s));
 
 function Set#Empty<T>(): Set T;
-axiom (forall<T> o: T :: { Set#Empty()[o] } !Set#Empty()[o]);
-axiom (forall<T> s: Set T :: { Set#Card(s) }
+axiom {:root} (forall<T> o: T :: { Set#Empty()[o] } !Set#Empty()[o]);
+axiom {:root} (forall<T> s: Set T :: { Set#Card(s) }
   (Set#Card(s) == 0 <==> s == Set#Empty()) &&
   (Set#Card(s) != 0 ==> (exists x: T :: s[x])));
 
@@ -649,30 +659,30 @@ axiom (forall<T> s: Set T :: { Set#Card(s) }
 //axiom (forall<T> t: Ty :: { $Is(Set#Empty() : [T]bool, TSet(t)) } $Is(Set#Empty() : [T]bool, TSet(t)));
 
 function Set#Singleton<T>(T): Set T;
-axiom (forall<T> r: T :: { Set#Singleton(r) } Set#Singleton(r)[r]);
-axiom (forall<T> r: T, o: T :: { Set#Singleton(r)[o] } Set#Singleton(r)[o] <==> r == o);
-axiom (forall<T> r: T :: { Set#Card(Set#Singleton(r)) } Set#Card(Set#Singleton(r)) == 1);
+axiom {:root} (forall<T> r: T :: { Set#Singleton(r) } Set#Singleton(r)[r]);
+axiom {:root} (forall<T> r: T, o: T :: { Set#Singleton(r)[o] } Set#Singleton(r)[o] <==> r == o);
+axiom {:root} (forall<T> r: T :: { Set#Card(Set#Singleton(r)) } Set#Card(Set#Singleton(r)) == 1);
 
 function Set#UnionOne<T>(Set T, T): Set T;
-axiom (forall<T> a: Set T, x: T, o: T :: { Set#UnionOne(a,x)[o] }
+axiom {:root} (forall<T> a: Set T, x: T, o: T :: { Set#UnionOne(a,x)[o] }
   Set#UnionOne(a,x)[o] <==> o == x || a[o]);
-axiom (forall<T> a: Set T, x: T :: { Set#UnionOne(a, x) }
+axiom {:root} (forall<T> a: Set T, x: T :: { Set#UnionOne(a, x) }
   Set#UnionOne(a, x)[x]);
-axiom (forall<T> a: Set T, x: T, y: T :: { Set#UnionOne(a, x), a[y] }
+axiom {:root} (forall<T> a: Set T, x: T, y: T :: { Set#UnionOne(a, x), a[y] }
   a[y] ==> Set#UnionOne(a, x)[y]);
-axiom (forall<T> a: Set T, x: T :: { Set#Card(Set#UnionOne(a, x)) }
+axiom {:root} (forall<T> a: Set T, x: T :: { Set#Card(Set#UnionOne(a, x)) }
   a[x] ==> Set#Card(Set#UnionOne(a, x)) == Set#Card(a));
-axiom (forall<T> a: Set T, x: T :: { Set#Card(Set#UnionOne(a, x)) }
+axiom {:root} (forall<T> a: Set T, x: T :: { Set#Card(Set#UnionOne(a, x)) }
   !a[x] ==> Set#Card(Set#UnionOne(a, x)) == Set#Card(a) + 1);
 
 function Set#Union<T>(Set T, Set T): Set T;
-axiom (forall<T> a: Set T, b: Set T, o: T :: { Set#Union(a,b)[o] }
+axiom {:root} (forall<T> a: Set T, b: Set T, o: T :: { Set#Union(a,b)[o] }
   Set#Union(a,b)[o] <==> a[o] || b[o]);
-axiom (forall<T> a, b: Set T, y: T :: { Set#Union(a, b), a[y] }
+axiom {:root} (forall<T> a, b: Set T, y: T :: { Set#Union(a, b), a[y] }
   a[y] ==> Set#Union(a, b)[y]);
-axiom (forall<T> a, b: Set T, y: T :: { Set#Union(a, b), b[y] }
+axiom {:root} (forall<T> a, b: Set T, y: T :: { Set#Union(a, b), b[y] }
   b[y] ==> Set#Union(a, b)[y]);
-axiom (forall<T> a, b: Set T :: { Set#Union(a, b) }
+axiom {:root} (forall<T> a, b: Set T :: { Set#Union(a, b) }
   Set#Disjoint(a, b) ==>
     Set#Difference(Set#Union(a, b), a) == b &&
     Set#Difference(Set#Union(a, b), b) == a);
@@ -682,26 +692,26 @@ axiom (forall<T> a, b: Set T :: { Set#Union(a, b) }
 //     Set#Card(Set#Union(a, b)) == Set#Card(a) + Set#Card(b));
 
 function Set#Intersection<T>(Set T, Set T): Set T;
-axiom (forall<T> a: Set T, b: Set T, o: T :: { Set#Intersection(a,b)[o] }
+axiom {:root} (forall<T> a: Set T, b: Set T, o: T :: { Set#Intersection(a,b)[o] }
   Set#Intersection(a,b)[o] <==> a[o] && b[o]);
 
-axiom (forall<T> a, b: Set T :: { Set#Union(Set#Union(a, b), b) }
+axiom {:root} (forall<T> a, b: Set T :: { Set#Union(Set#Union(a, b), b) }
   Set#Union(Set#Union(a, b), b) == Set#Union(a, b));
-axiom (forall<T> a, b: Set T :: { Set#Union(a, Set#Union(a, b)) }
+axiom {:root} (forall<T> a, b: Set T :: { Set#Union(a, Set#Union(a, b)) }
   Set#Union(a, Set#Union(a, b)) == Set#Union(a, b));
-axiom (forall<T> a, b: Set T :: { Set#Intersection(Set#Intersection(a, b), b) }
+axiom {:root} (forall<T> a, b: Set T :: { Set#Intersection(Set#Intersection(a, b), b) }
   Set#Intersection(Set#Intersection(a, b), b) == Set#Intersection(a, b));
-axiom (forall<T> a, b: Set T :: { Set#Intersection(a, Set#Intersection(a, b)) }
+axiom {:root} (forall<T> a, b: Set T :: { Set#Intersection(a, Set#Intersection(a, b)) }
   Set#Intersection(a, Set#Intersection(a, b)) == Set#Intersection(a, b));
-axiom (forall<T> a, b: Set T :: { Set#Card(Set#Union(a, b)) }{ Set#Card(Set#Intersection(a, b)) }
+axiom {:root} (forall<T> a, b: Set T :: { Set#Card(Set#Union(a, b)) }{ Set#Card(Set#Intersection(a, b)) }
   Set#Card(Set#Union(a, b)) + Set#Card(Set#Intersection(a, b)) == Set#Card(a) + Set#Card(b));
 
 function Set#Difference<T>(Set T, Set T): Set T;
-axiom (forall<T> a: Set T, b: Set T, o: T :: { Set#Difference(a,b)[o] }
+axiom {:root} (forall<T> a: Set T, b: Set T, o: T :: { Set#Difference(a,b)[o] }
   Set#Difference(a,b)[o] <==> a[o] && !b[o]);
-axiom (forall<T> a, b: Set T, y: T :: { Set#Difference(a, b), b[y] }
+axiom {:root} (forall<T> a, b: Set T, y: T :: { Set#Difference(a, b), b[y] }
   b[y] ==> !Set#Difference(a, b)[y] );
-axiom (forall<T> a, b: Set T ::
+axiom {:root} (forall<T> a, b: Set T ::
   { Set#Card(Set#Difference(a, b)) }
   Set#Card(Set#Difference(a, b)) + Set#Card(Set#Difference(b, a))
   + Set#Card(Set#Intersection(a, b))
@@ -709,7 +719,7 @@ axiom (forall<T> a, b: Set T ::
   Set#Card(Set#Difference(a, b)) == Set#Card(a) - Set#Card(Set#Intersection(a, b)));
 
 function Set#Subset<T>(Set T, Set T): bool;
-axiom(forall<T> a: Set T, b: Set T :: { Set#Subset(a,b) }
+axiom {:root} (forall<T> a: Set T, b: Set T :: { Set#Subset(a,b) }
   Set#Subset(a,b) <==> (forall o: T :: {a[o]} {b[o]} a[o] ==> b[o]));
 // axiom(forall<T> a: Set T, b: Set T ::
 //   { Set#Subset(a,b), Set#Card(a), Set#Card(b) }  // very restrictive trigger
@@ -717,13 +727,13 @@ axiom(forall<T> a: Set T, b: Set T :: { Set#Subset(a,b) }
 
 
 function Set#Equal<T>(Set T, Set T): bool;
-axiom(forall<T> a: Set T, b: Set T :: { Set#Equal(a,b) }
+axiom {:root} (forall<T> a: Set T, b: Set T :: { Set#Equal(a,b) }
   Set#Equal(a,b) <==> (forall o: T :: {a[o]} {b[o]} a[o] <==> b[o]));
-axiom(forall<T> a: Set T, b: Set T :: { Set#Equal(a,b) }  // extensionality axiom for sets
+axiom {:root} (forall<T> a: Set T, b: Set T :: { Set#Equal(a,b) }  // extensionality axiom for sets
   Set#Equal(a,b) ==> a == b);
 
 function Set#Disjoint<T>(Set T, Set T): bool;
-axiom (forall<T> a: Set T, b: Set T :: { Set#Disjoint(a,b) }
+axiom {:root} (forall<T> a: Set T, b: Set T :: { Set#Disjoint(a,b) }
   Set#Disjoint(a,b) <==> (forall o: T :: {a[o]} {b[o]} !a[o] || !b[o]));
 
 // ---------------------------------------------------------------
@@ -733,64 +743,64 @@ axiom (forall<T> a: Set T, b: Set T :: { Set#Disjoint(a,b) }
 type ISet T = [T]bool;
 
 function ISet#Empty<T>(): Set T;
-axiom (forall<T> o: T :: { ISet#Empty()[o] } !ISet#Empty()[o]);
+axiom {:root} (forall<T> o: T :: { ISet#Empty()[o] } !ISet#Empty()[o]);
 
 // the empty set could be of anything
 //axiom (forall<T> t: Ty :: { $Is(ISet#Empty() : [T]bool, TISet(t)) } $Is(ISet#Empty() : [T]bool, TISet(t)));
 
 
 function ISet#UnionOne<T>(ISet T, T): ISet T;
-axiom (forall<T> a: ISet T, x: T, o: T :: { ISet#UnionOne(a,x)[o] }
+axiom {:root} (forall<T> a: ISet T, x: T, o: T :: { ISet#UnionOne(a,x)[o] }
   ISet#UnionOne(a,x)[o] <==> o == x || a[o]);
-axiom (forall<T> a: ISet T, x: T :: { ISet#UnionOne(a, x) }
+axiom {:root} (forall<T> a: ISet T, x: T :: { ISet#UnionOne(a, x) }
   ISet#UnionOne(a, x)[x]);
-axiom (forall<T> a: ISet T, x: T, y: T :: { ISet#UnionOne(a, x), a[y] }
+axiom {:root} (forall<T> a: ISet T, x: T, y: T :: { ISet#UnionOne(a, x), a[y] }
   a[y] ==> ISet#UnionOne(a, x)[y]);
 
 function ISet#Union<T>(ISet T, ISet T): ISet T;
-axiom (forall<T> a: ISet T, b: ISet T, o: T :: { ISet#Union(a,b)[o] }
+axiom {:root} (forall<T> a: ISet T, b: ISet T, o: T :: { ISet#Union(a,b)[o] }
   ISet#Union(a,b)[o] <==> a[o] || b[o]);
-axiom (forall<T> a, b: ISet T, y: T :: { ISet#Union(a, b), a[y] }
+axiom {:root} (forall<T> a, b: ISet T, y: T :: { ISet#Union(a, b), a[y] }
   a[y] ==> ISet#Union(a, b)[y]);
-axiom (forall<T> a, b: Set T, y: T :: { ISet#Union(a, b), b[y] }
+axiom {:root} (forall<T> a, b: Set T, y: T :: { ISet#Union(a, b), b[y] }
   b[y] ==> ISet#Union(a, b)[y]);
-axiom (forall<T> a, b: ISet T :: { ISet#Union(a, b) }
+axiom {:root} (forall<T> a, b: ISet T :: { ISet#Union(a, b) }
   ISet#Disjoint(a, b) ==>
     ISet#Difference(ISet#Union(a, b), a) == b &&
     ISet#Difference(ISet#Union(a, b), b) == a);
 
 function ISet#Intersection<T>(ISet T, ISet T): ISet T;
-axiom (forall<T> a: ISet T, b: ISet T, o: T :: { ISet#Intersection(a,b)[o] }
+axiom {:root} (forall<T> a: ISet T, b: ISet T, o: T :: { ISet#Intersection(a,b)[o] }
   ISet#Intersection(a,b)[o] <==> a[o] && b[o]);
 
-axiom (forall<T> a, b: ISet T :: { ISet#Union(ISet#Union(a, b), b) }
+axiom {:root} (forall<T> a, b: ISet T :: { ISet#Union(ISet#Union(a, b), b) }
   ISet#Union(ISet#Union(a, b), b) == ISet#Union(a, b));
-axiom (forall<T> a, b: Set T :: { ISet#Union(a, ISet#Union(a, b)) }
+axiom {:root} (forall<T> a, b: Set T :: { ISet#Union(a, ISet#Union(a, b)) }
   ISet#Union(a, ISet#Union(a, b)) == ISet#Union(a, b));
-axiom (forall<T> a, b: ISet T :: { ISet#Intersection(ISet#Intersection(a, b), b) }
+axiom {:root} (forall<T> a, b: ISet T :: { ISet#Intersection(ISet#Intersection(a, b), b) }
   ISet#Intersection(ISet#Intersection(a, b), b) == ISet#Intersection(a, b));
-axiom (forall<T> a, b: ISet T :: { ISet#Intersection(a, ISet#Intersection(a, b)) }
+axiom {:root} (forall<T> a, b: ISet T :: { ISet#Intersection(a, ISet#Intersection(a, b)) }
   ISet#Intersection(a, ISet#Intersection(a, b)) == ISet#Intersection(a, b));
 
 
 function ISet#Difference<T>(ISet T, ISet T): ISet T;
-axiom (forall<T> a: ISet T, b: ISet T, o: T :: { ISet#Difference(a,b)[o] }
+axiom {:root} (forall<T> a: ISet T, b: ISet T, o: T :: { ISet#Difference(a,b)[o] }
   ISet#Difference(a,b)[o] <==> a[o] && !b[o]);
-axiom (forall<T> a, b: ISet T, y: T :: { ISet#Difference(a, b), b[y] }
+axiom {:root} (forall<T> a, b: ISet T, y: T :: { ISet#Difference(a, b), b[y] }
   b[y] ==> !ISet#Difference(a, b)[y] );
 
 function ISet#Subset<T>(ISet T, ISet T): bool;
-axiom(forall<T> a: ISet T, b: ISet T :: { ISet#Subset(a,b) }
+axiom {:root} (forall<T> a: ISet T, b: ISet T :: { ISet#Subset(a,b) }
   ISet#Subset(a,b) <==> (forall o: T :: {a[o]} {b[o]} a[o] ==> b[o]));
 
 function ISet#Equal<T>(ISet T, ISet T): bool;
-axiom(forall<T> a: ISet T, b: ISet T :: { ISet#Equal(a,b) }
+axiom {:root} (forall<T> a: ISet T, b: ISet T :: { ISet#Equal(a,b) }
   ISet#Equal(a,b) <==> (forall o: T :: {a[o]} {b[o]} a[o] <==> b[o]));
-axiom(forall<T> a: ISet T, b: ISet T :: { ISet#Equal(a,b) }  // extensionality axiom for sets
+axiom {:root} (forall<T> a: ISet T, b: ISet T :: { ISet#Equal(a,b) }  // extensionality axiom for sets
   ISet#Equal(a,b) ==> a == b);
 
 function ISet#Disjoint<T>(ISet T, ISet T): bool;
-axiom (forall<T> a: ISet T, b: ISet T :: { ISet#Disjoint(a,b) }
+axiom {:root} (forall<T> a: ISet T, b: ISet T :: { ISet#Disjoint(a,b) }
   ISet#Disjoint(a,b) <==> (forall o: T :: {a[o]} {b[o]} !a[o] || !b[o]));
 
 // ---------------------------------------------------------------
@@ -798,79 +808,79 @@ axiom (forall<T> a: ISet T, b: ISet T :: { ISet#Disjoint(a,b) }
 // ---------------------------------------------------------------
 
 function Math#min(a: int, b: int): int;
-axiom (forall a: int, b: int :: { Math#min(a, b) } a <= b <==> Math#min(a, b) == a);
-axiom (forall a: int, b: int :: { Math#min(a, b) } b <= a <==> Math#min(a, b) == b);
-axiom (forall a: int, b: int :: { Math#min(a, b) } Math#min(a, b) == a || Math#min(a, b) == b);
+axiom {:root} (forall a: int, b: int :: { Math#min(a, b) } a <= b <==> Math#min(a, b) == a);
+axiom {:root} (forall a: int, b: int :: { Math#min(a, b) } b <= a <==> Math#min(a, b) == b);
+axiom {:root} (forall a: int, b: int :: { Math#min(a, b) } Math#min(a, b) == a || Math#min(a, b) == b);
 
 function Math#clip(a: int): int;
-axiom (forall a: int :: { Math#clip(a) } 0 <= a ==> Math#clip(a) == a);
-axiom (forall a: int :: { Math#clip(a) } a < 0  ==> Math#clip(a) == 0);
+axiom {:root} (forall a: int :: { Math#clip(a) } 0 <= a ==> Math#clip(a) == a);
+axiom {:root} (forall a: int :: { Math#clip(a) } a < 0  ==> Math#clip(a) == 0);
 
 type MultiSet T = [T]int;
 
 function $IsGoodMultiSet<T>(ms: MultiSet T): bool;
 // ints are non-negative, used after havocing, and for conversion from sequences to multisets.
-axiom (forall<T> ms: MultiSet T :: { $IsGoodMultiSet(ms) }
+axiom {:root} (forall<T> ms: MultiSet T :: { $IsGoodMultiSet(ms) }
   $IsGoodMultiSet(ms) <==>
   (forall bx: T :: { ms[bx] } 0 <= ms[bx] && ms[bx] <= MultiSet#Card(ms)));
 
 function MultiSet#Card<T>(MultiSet T): int;
-axiom (forall<T> s: MultiSet T :: { MultiSet#Card(s) } 0 <= MultiSet#Card(s));
-axiom (forall<T> s: MultiSet T, x: T, n: int :: { MultiSet#Card(s[x := n]) }
+axiom {:root} (forall<T> s: MultiSet T :: { MultiSet#Card(s) } 0 <= MultiSet#Card(s));
+axiom {:root} (forall<T> s: MultiSet T, x: T, n: int :: { MultiSet#Card(s[x := n]) }
   0 <= n ==> MultiSet#Card(s[x := n]) == MultiSet#Card(s) - s[x] + n);
 
 function MultiSet#Empty<T>(): MultiSet T;
-axiom (forall<T> o: T :: { MultiSet#Empty()[o] } MultiSet#Empty()[o] == 0);
-axiom (forall<T> s: MultiSet T :: { MultiSet#Card(s) }
+axiom {:root} (forall<T> o: T :: { MultiSet#Empty()[o] } MultiSet#Empty()[o] == 0);
+axiom {:root} (forall<T> s: MultiSet T :: { MultiSet#Card(s) }
   (MultiSet#Card(s) == 0 <==> s == MultiSet#Empty()) &&
   (MultiSet#Card(s) != 0 ==> (exists x: T :: 0 < s[x])));
 
 function MultiSet#Singleton<T>(T): MultiSet T;
-axiom (forall<T> r: T, o: T :: { MultiSet#Singleton(r)[o] } (MultiSet#Singleton(r)[o] == 1 <==> r == o) &&
+axiom {:root} (forall<T> r: T, o: T :: { MultiSet#Singleton(r)[o] } (MultiSet#Singleton(r)[o] == 1 <==> r == o) &&
                                                             (MultiSet#Singleton(r)[o] == 0 <==> r != o));
-axiom (forall<T> r: T :: { MultiSet#Singleton(r) } MultiSet#Singleton(r) == MultiSet#UnionOne(MultiSet#Empty(), r));
+axiom {:root} (forall<T> r: T :: { MultiSet#Singleton(r) } MultiSet#Singleton(r) == MultiSet#UnionOne(MultiSet#Empty(), r));
 
 function MultiSet#UnionOne<T>(MultiSet T, T): MultiSet T;
 // pure containment axiom (in the original multiset or is the added element)
-axiom (forall<T> a: MultiSet T, x: T, o: T :: { MultiSet#UnionOne(a,x)[o] }
+axiom {:root} (forall<T> a: MultiSet T, x: T, o: T :: { MultiSet#UnionOne(a,x)[o] }
   0 < MultiSet#UnionOne(a,x)[o] <==> o == x || 0 < a[o]);
 // union-ing increases count by one
-axiom (forall<T> a: MultiSet T, x: T :: { MultiSet#UnionOne(a, x) }
+axiom {:root} (forall<T> a: MultiSet T, x: T :: { MultiSet#UnionOne(a, x) }
   MultiSet#UnionOne(a, x)[x] == a[x] + 1);
 // non-decreasing
-axiom (forall<T> a: MultiSet T, x: T, y: T :: { MultiSet#UnionOne(a, x), a[y] }
+axiom {:root} (forall<T> a: MultiSet T, x: T, y: T :: { MultiSet#UnionOne(a, x), a[y] }
   0 < a[y] ==> 0 < MultiSet#UnionOne(a, x)[y]);
 // other elements unchanged
-axiom (forall<T> a: MultiSet T, x: T, y: T :: { MultiSet#UnionOne(a, x), a[y] }
+axiom {:root} (forall<T> a: MultiSet T, x: T, y: T :: { MultiSet#UnionOne(a, x), a[y] }
   x != y ==> a[y] == MultiSet#UnionOne(a, x)[y]);
-axiom (forall<T> a: MultiSet T, x: T :: { MultiSet#Card(MultiSet#UnionOne(a, x)) }
+axiom {:root} (forall<T> a: MultiSet T, x: T :: { MultiSet#Card(MultiSet#UnionOne(a, x)) }
   MultiSet#Card(MultiSet#UnionOne(a, x)) == MultiSet#Card(a) + 1);
 
 
 function MultiSet#Union<T>(MultiSet T, MultiSet T): MultiSet T;
 // union-ing is the sum of the contents
-axiom (forall<T> a: MultiSet T, b: MultiSet T, o: T :: { MultiSet#Union(a,b)[o] }
+axiom {:root} (forall<T> a: MultiSet T, b: MultiSet T, o: T :: { MultiSet#Union(a,b)[o] }
   MultiSet#Union(a,b)[o] == a[o] + b[o]);
-axiom (forall<T> a: MultiSet T, b: MultiSet T :: { MultiSet#Card(MultiSet#Union(a,b)) }
+axiom {:root} (forall<T> a: MultiSet T, b: MultiSet T :: { MultiSet#Card(MultiSet#Union(a,b)) }
   MultiSet#Card(MultiSet#Union(a,b)) == MultiSet#Card(a) + MultiSet#Card(b));
 
 function MultiSet#Intersection<T>(MultiSet T, MultiSet T): MultiSet T;
-axiom (forall<T> a: MultiSet T, b: MultiSet T, o: T :: { MultiSet#Intersection(a,b)[o] }
+axiom {:root} (forall<T> a: MultiSet T, b: MultiSet T, o: T :: { MultiSet#Intersection(a,b)[o] }
   MultiSet#Intersection(a,b)[o] == Math#min(a[o],  b[o]));
 
 // left and right pseudo-idempotence
-axiom (forall<T> a, b: MultiSet T :: { MultiSet#Intersection(MultiSet#Intersection(a, b), b) }
+axiom {:root} (forall<T> a, b: MultiSet T :: { MultiSet#Intersection(MultiSet#Intersection(a, b), b) }
   MultiSet#Intersection(MultiSet#Intersection(a, b), b) == MultiSet#Intersection(a, b));
-axiom (forall<T> a, b: MultiSet T :: { MultiSet#Intersection(a, MultiSet#Intersection(a, b)) }
+axiom {:root} (forall<T> a, b: MultiSet T :: { MultiSet#Intersection(a, MultiSet#Intersection(a, b)) }
   MultiSet#Intersection(a, MultiSet#Intersection(a, b)) == MultiSet#Intersection(a, b));
 
 // multiset difference, a - b. clip() makes it positive.
 function MultiSet#Difference<T>(MultiSet T, MultiSet T): MultiSet T;
-axiom (forall<T> a: MultiSet T, b: MultiSet T, o: T :: { MultiSet#Difference(a,b)[o] }
+axiom {:root} (forall<T> a: MultiSet T, b: MultiSet T, o: T :: { MultiSet#Difference(a,b)[o] }
   MultiSet#Difference(a,b)[o] == Math#clip(a[o] - b[o]));
-axiom (forall<T> a, b: MultiSet T, y: T :: { MultiSet#Difference(a, b), b[y], a[y] }
+axiom {:root} (forall<T> a, b: MultiSet T, y: T :: { MultiSet#Difference(a, b), b[y], a[y] }
   a[y] <= b[y] ==> MultiSet#Difference(a, b)[y] == 0 );
-axiom (forall<T> a, b: MultiSet T ::
+axiom {:root} (forall<T> a, b: MultiSet T ::
   { MultiSet#Card(MultiSet#Difference(a, b)) }
   MultiSet#Card(MultiSet#Difference(a, b)) + MultiSet#Card(MultiSet#Difference(b, a))
   + 2 * MultiSet#Card(MultiSet#Intersection(a, b))
@@ -879,56 +889,56 @@ axiom (forall<T> a, b: MultiSet T ::
 
 // multiset subset means a must have at most as many of each element as b
 function MultiSet#Subset<T>(MultiSet T, MultiSet T): bool;
-axiom(forall<T> a: MultiSet T, b: MultiSet T :: { MultiSet#Subset(a,b) }
+axiom {:root} (forall<T> a: MultiSet T, b: MultiSet T :: { MultiSet#Subset(a,b) }
   MultiSet#Subset(a,b) <==> (forall o: T :: {a[o]} {b[o]} a[o] <= b[o]));
 
 function MultiSet#Equal<T>(MultiSet T, MultiSet T): bool;
-axiom(forall<T> a: MultiSet T, b: MultiSet T :: { MultiSet#Equal(a,b) }
+axiom {:root} (forall<T> a: MultiSet T, b: MultiSet T :: { MultiSet#Equal(a,b) }
   MultiSet#Equal(a,b) <==> (forall o: T :: {a[o]} {b[o]} a[o] == b[o]));
 // extensionality axiom for multisets
-axiom(forall<T> a: MultiSet T, b: MultiSet T :: { MultiSet#Equal(a,b) }
+axiom {:root} (forall<T> a: MultiSet T, b: MultiSet T :: { MultiSet#Equal(a,b) }
   MultiSet#Equal(a,b) ==> a == b);
 
 function MultiSet#Disjoint<T>(MultiSet T, MultiSet T): bool;
-axiom (forall<T> a: MultiSet T, b: MultiSet T :: { MultiSet#Disjoint(a,b) }
+axiom {:root} (forall<T> a: MultiSet T, b: MultiSet T :: { MultiSet#Disjoint(a,b) }
   MultiSet#Disjoint(a,b) <==> (forall o: T :: {a[o]} {b[o]} a[o] == 0 || b[o] == 0));
 
 // conversion to a multiset. each element in the original set has duplicity 1.
 function MultiSet#FromSet<T>(Set T): MultiSet T;
-axiom (forall<T> s: Set T, a: T :: { MultiSet#FromSet(s)[a] }
+axiom {:root} (forall<T> s: Set T, a: T :: { MultiSet#FromSet(s)[a] }
   (MultiSet#FromSet(s)[a] == 0 <==> !s[a]) &&
   (MultiSet#FromSet(s)[a] == 1 <==> s[a]));
-axiom (forall<T> s: Set T :: { MultiSet#Card(MultiSet#FromSet(s)) }
+axiom {:root} (forall<T> s: Set T :: { MultiSet#Card(MultiSet#FromSet(s)) }
   MultiSet#Card(MultiSet#FromSet(s)) == Set#Card(s));
 
 // conversion to a multiset, from a sequence.
 function MultiSet#FromSeq<T>(Seq T): MultiSet T;
 // conversion produces a good map.
-axiom (forall<T> s: Seq T :: { MultiSet#FromSeq(s) } $IsGoodMultiSet(MultiSet#FromSeq(s)) );
+axiom {:root} (forall<T> s: Seq T :: { MultiSet#FromSeq(s) } $IsGoodMultiSet(MultiSet#FromSeq(s)) );
 // cardinality axiom
-axiom (forall<T> s: Seq T ::
+axiom {:root} (forall<T> s: Seq T ::
   { MultiSet#Card(MultiSet#FromSeq(s)) }
     MultiSet#Card(MultiSet#FromSeq(s)) == Seq#Length(s));
 // building axiom
-axiom (forall<T> s: Seq T, v: T ::
+axiom {:root} (forall<T> s: Seq T, v: T ::
   { MultiSet#FromSeq(Seq#Build(s, v)) }
     MultiSet#FromSeq(Seq#Build(s, v)) == MultiSet#UnionOne(MultiSet#FromSeq(s), v)
   );
-axiom (forall<T> :: MultiSet#FromSeq(Seq#Empty(): Seq T) == MultiSet#Empty(): MultiSet T);
+axiom {:root} (forall<T> :: MultiSet#FromSeq(Seq#Empty(): Seq T) == MultiSet#Empty(): MultiSet T);
 
 // concatenation axiom
-axiom (forall<T> a: Seq T, b: Seq T ::
+axiom {:root} (forall<T> a: Seq T, b: Seq T ::
   { MultiSet#FromSeq(Seq#Append(a, b)) }
     MultiSet#FromSeq(Seq#Append(a, b)) == MultiSet#Union(MultiSet#FromSeq(a), MultiSet#FromSeq(b)) );
 
 // update axiom
-axiom (forall<T> s: Seq T, i: int, v: T, x: T ::
+axiom {:root} (forall<T> s: Seq T, i: int, v: T, x: T ::
   { MultiSet#FromSeq(Seq#Update(s, i, v))[x] }
     0 <= i && i < Seq#Length(s) ==>
     MultiSet#FromSeq(Seq#Update(s, i, v))[x] ==
       MultiSet#Union(MultiSet#Difference(MultiSet#FromSeq(s), MultiSet#Singleton(Seq#Index(s,i))), MultiSet#Singleton(v))[x] );
   // i.e. MS(Update(s, i, v)) == MS(s) - {{s[i]}} + {{v}}
-axiom (forall<T> s: Seq T, x: T :: { MultiSet#FromSeq(s)[x] }
+axiom {:root} (forall<T> s: Seq T, x: T :: { MultiSet#FromSeq(s)[x] }
   (exists i : int :: { Seq#Index(s,i) } 0 <= i && i < Seq#Length(s) && x == Seq#Index(s,i)) <==> 0 < MultiSet#FromSeq(s)[x] );
 
 // ---------------------------------------------------------------
@@ -938,11 +948,11 @@ axiom (forall<T> s: Seq T, x: T :: { MultiSet#FromSeq(s)[x] }
 type Seq T;
 
 function Seq#Length<T>(Seq T): int;
-axiom (forall<T> s: Seq T :: { Seq#Length(s) } 0 <= Seq#Length(s));
+axiom {:root} (forall<T> s: Seq T :: { Seq#Length(s) } 0 <= Seq#Length(s));
 
 function Seq#Empty<T>(): Seq T;
-axiom (forall<T> :: { Seq#Empty(): Seq T } Seq#Length(Seq#Empty(): Seq T) == 0);
-axiom (forall<T> s: Seq T :: { Seq#Length(s) }
+axiom {:root} (forall<T> :: { Seq#Empty(): Seq T } Seq#Length(Seq#Empty(): Seq T) == 0);
+axiom {:root} (forall<T> s: Seq T :: { Seq#Length(s) }
   (Seq#Length(s) == 0 ==> s == Seq#Empty())
 // The following would be a nice fact to include, because it would enable verifying the
 // GenericPick.SeqPick* methods in Test/dafny0/SmallTests.dfy.  However, it substantially
@@ -955,102 +965,102 @@ axiom (forall<T> s: Seq T :: { Seq#Length(s) }
 //axiom (forall<T> t: Ty :: {$Is(Seq#Empty(): Seq T, TSeq(t))} $Is(Seq#Empty(): Seq T, TSeq(t)));
 
 function Seq#Singleton<T>(T): Seq T;
-axiom (forall<T> t: T :: { Seq#Length(Seq#Singleton(t)) } Seq#Length(Seq#Singleton(t)) == 1);
+axiom {:root} (forall<T> t: T :: { Seq#Length(Seq#Singleton(t)) } Seq#Length(Seq#Singleton(t)) == 1);
 
 function Seq#Build<T>(s: Seq T, val: T): Seq T;
 function Seq#Build_inv0<T>(s: Seq T) : Seq T;
 function Seq#Build_inv1<T>(s: Seq T) : T;
-axiom (forall<T> s: Seq T, val: T ::
+axiom {:root} (forall<T> s: Seq T, val: T ::
   { Seq#Build(s, val) }
   Seq#Build_inv0(Seq#Build(s, val)) == s &&
   Seq#Build_inv1(Seq#Build(s, val)) == val);
 
-axiom (forall<T> s: Seq T, v: T ::
+axiom {:root} (forall<T> s: Seq T, v: T ::
   { Seq#Build(s,v) }
   Seq#Length(Seq#Build(s,v)) == 1 + Seq#Length(s));
-axiom (forall<T> s: Seq T, i: int, v: T :: { Seq#Index(Seq#Build(s,v), i) }
+axiom {:root} (forall<T> s: Seq T, i: int, v: T :: { Seq#Index(Seq#Build(s,v), i) }
   (i == Seq#Length(s) ==> Seq#Index(Seq#Build(s,v), i) == v) &&
   (i != Seq#Length(s) ==> Seq#Index(Seq#Build(s,v), i) == Seq#Index(s, i)));
 
 // Build preserves $Is
-axiom (forall s: Seq Box, bx: Box, t: Ty :: { $Is(Seq#Build(s,bx),TSeq(t)) }
+axiom {:root} (forall s: Seq Box, bx: Box, t: Ty :: { $Is(Seq#Build(s,bx),TSeq(t)) }
     $Is(s,TSeq(t)) && $IsBox(bx,t) ==> $Is(Seq#Build(s,bx),TSeq(t)));
 
 function Seq#Create(ty: Ty, heap: Heap, len: int, init: HandleType): Seq Box;
-axiom (forall ty: Ty, heap: Heap, len: int, init: HandleType ::
+axiom {:root} (forall ty: Ty, heap: Heap, len: int, init: HandleType ::
   { Seq#Length(Seq#Create(ty, heap, len, init): Seq Box) }
   $IsGoodHeap(heap) && 0 <= len ==>
   Seq#Length(Seq#Create(ty, heap, len, init): Seq Box) == len);
-axiom (forall ty: Ty, heap: Heap, len: int, init: HandleType, i: int ::
+axiom {:root} (forall ty: Ty, heap: Heap, len: int, init: HandleType, i: int ::
   { Seq#Index(Seq#Create(ty, heap, len, init), i) }
   $IsGoodHeap(heap) && 0 <= i && i < len ==>
   Seq#Index(Seq#Create(ty, heap, len, init), i) == Apply1(TInt, TSeq(ty), heap, init, $Box(i)));
 
 function Seq#Append<T>(Seq T, Seq T): Seq T;
-axiom (forall<T> s0: Seq T, s1: Seq T :: { Seq#Length(Seq#Append(s0,s1)) }
+axiom {:root} (forall<T> s0: Seq T, s1: Seq T :: { Seq#Length(Seq#Append(s0,s1)) }
   Seq#Length(Seq#Append(s0,s1)) == Seq#Length(s0) + Seq#Length(s1));
 
 function Seq#Index<T>(Seq T, int): T;
-axiom (forall<T> t: T :: { Seq#Index(Seq#Singleton(t), 0) } Seq#Index(Seq#Singleton(t), 0) == t);
-axiom (forall<T> s0: Seq T, s1: Seq T, n: int :: { Seq#Index(Seq#Append(s0,s1), n) }
+axiom {:root} (forall<T> t: T :: { Seq#Index(Seq#Singleton(t), 0) } Seq#Index(Seq#Singleton(t), 0) == t);
+axiom {:root} (forall<T> s0: Seq T, s1: Seq T, n: int :: { Seq#Index(Seq#Append(s0,s1), n) }
   (n < Seq#Length(s0) ==> Seq#Index(Seq#Append(s0,s1), n) == Seq#Index(s0, n)) &&
   (Seq#Length(s0) <= n ==> Seq#Index(Seq#Append(s0,s1), n) == Seq#Index(s1, n - Seq#Length(s0))));
 
 function Seq#Update<T>(Seq T, int, T): Seq T;
-axiom (forall<T> s: Seq T, i: int, v: T :: { Seq#Length(Seq#Update(s,i,v)) }
+axiom {:root} (forall<T> s: Seq T, i: int, v: T :: { Seq#Length(Seq#Update(s,i,v)) }
   0 <= i && i < Seq#Length(s) ==> Seq#Length(Seq#Update(s,i,v)) == Seq#Length(s));
-axiom (forall<T> s: Seq T, i: int, v: T, n: int :: { Seq#Index(Seq#Update(s,i,v),n) }
+axiom {:root} (forall<T> s: Seq T, i: int, v: T, n: int :: { Seq#Index(Seq#Update(s,i,v),n) }
   0 <= n && n < Seq#Length(s) ==>
     (i == n ==> Seq#Index(Seq#Update(s,i,v),n) == v) &&
     (i != n ==> Seq#Index(Seq#Update(s,i,v),n) == Seq#Index(s,n)));
 
 function Seq#Contains<T>(Seq T, T): bool;
-axiom (forall<T> s: Seq T, x: T :: { Seq#Contains(s,x) }
+axiom {:root} (forall<T> s: Seq T, x: T :: { Seq#Contains(s,x) }
   Seq#Contains(s,x) <==>
     (exists i: int :: { Seq#Index(s,i) } 0 <= i && i < Seq#Length(s) && Seq#Index(s,i) == x));
-axiom (forall<T> x: T ::
+axiom {:root} (forall<T> x: T ::
   { Seq#Contains(Seq#Empty(), x) }
   !Seq#Contains(Seq#Empty(), x));
 
-axiom (forall<T> s0: Seq T, s1: Seq T, x: T ::
+axiom {:root} (forall<T> s0: Seq T, s1: Seq T, x: T ::
   { Seq#Contains(Seq#Append(s0, s1), x) }
   Seq#Contains(Seq#Append(s0, s1), x) <==>
     Seq#Contains(s0, x) || Seq#Contains(s1, x));
 
-axiom (forall<T> s: Seq T, v: T, x: T ::  // needed to prove things like '4 in [2,3,4]', see method TestSequences0 in SmallTests.dfy
+axiom {:root} (forall<T> s: Seq T, v: T, x: T ::  // needed to prove things like '4 in [2,3,4]', see method TestSequences0 in SmallTests.dfy
   { Seq#Contains(Seq#Build(s, v), x) }
     Seq#Contains(Seq#Build(s, v), x) <==> (v == x || Seq#Contains(s, x)));
 
-axiom (forall<T> s: Seq T, n: int, x: T ::
+axiom {:root} (forall<T> s: Seq T, n: int, x: T ::
   { Seq#Contains(Seq#Take(s, n), x) }
   Seq#Contains(Seq#Take(s, n), x) <==>
     (exists i: int :: { Seq#Index(s, i) }
       0 <= i && i < n && i < Seq#Length(s) && Seq#Index(s, i) == x));
-axiom (forall<T> s: Seq T, n: int, x: T ::
+axiom {:root} (forall<T> s: Seq T, n: int, x: T ::
   { Seq#Contains(Seq#Drop(s, n), x) }
   Seq#Contains(Seq#Drop(s, n), x) <==>
     (exists i: int :: { Seq#Index(s, i) }
       0 <= n && n <= i && i < Seq#Length(s) && Seq#Index(s, i) == x));
 
 function Seq#Equal<T>(Seq T, Seq T): bool;
-axiom (forall<T> s0: Seq T, s1: Seq T :: { Seq#Equal(s0,s1) }
+axiom {:root} (forall<T> s0: Seq T, s1: Seq T :: { Seq#Equal(s0,s1) }
   Seq#Equal(s0,s1) <==>
     Seq#Length(s0) == Seq#Length(s1) &&
     (forall j: int :: { Seq#Index(s0,j) } { Seq#Index(s1,j) }
         0 <= j && j < Seq#Length(s0) ==> Seq#Index(s0,j) == Seq#Index(s1,j)));
-axiom (forall<T> a: Seq T, b: Seq T :: { Seq#Equal(a,b) }  // extensionality axiom for sequences
+axiom {:root} (forall<T> a: Seq T, b: Seq T :: { Seq#Equal(a,b) }  // extensionality axiom for sequences
   Seq#Equal(a,b) ==> a == b);
 
 function Seq#SameUntil<T>(Seq T, Seq T, int): bool;
-axiom (forall<T> s0: Seq T, s1: Seq T, n: int :: { Seq#SameUntil(s0,s1,n) }
+axiom {:root} (forall<T> s0: Seq T, s1: Seq T, n: int :: { Seq#SameUntil(s0,s1,n) }
   Seq#SameUntil(s0,s1,n) <==>
     (forall j: int :: { Seq#Index(s0,j) } { Seq#Index(s1,j) }
         0 <= j && j < n ==> Seq#Index(s0,j) == Seq#Index(s1,j)));
 
 function Seq#Take<T>(s: Seq T, howMany: int): Seq T;
-axiom (forall<T> s: Seq T, n: int :: { Seq#Length(Seq#Take(s,n)) }
+axiom {:root} (forall<T> s: Seq T, n: int :: { Seq#Length(Seq#Take(s,n)) }
   0 <= n && n <= Seq#Length(s) ==> Seq#Length(Seq#Take(s,n)) == n);
-axiom (forall<T> s: Seq T, n: int, j: int ::
+axiom {:root} (forall<T> s: Seq T, n: int, j: int ::
   {:weight 25}
   { Seq#Index(Seq#Take(s,n), j) }
   { Seq#Index(s, j), Seq#Take(s,n) }
@@ -1058,20 +1068,20 @@ axiom (forall<T> s: Seq T, n: int, j: int ::
     Seq#Index(Seq#Take(s,n), j) == Seq#Index(s, j));
 
 function Seq#Drop<T>(s: Seq T, howMany: int): Seq T;
-axiom (forall<T> s: Seq T, n: int :: { Seq#Length(Seq#Drop(s,n)) }
+axiom {:root} (forall<T> s: Seq T, n: int :: { Seq#Length(Seq#Drop(s,n)) }
   0 <= n && n <= Seq#Length(s) ==> Seq#Length(Seq#Drop(s,n)) == Seq#Length(s) - n);
-axiom (forall<T> s: Seq T, n: int, j: int ::
+axiom {:root} (forall<T> s: Seq T, n: int, j: int ::
   {:weight 25}
   { Seq#Index(Seq#Drop(s,n), j) }
   0 <= n && 0 <= j && j < Seq#Length(s)-n ==>
     Seq#Index(Seq#Drop(s,n), j) == Seq#Index(s, j+n));
-axiom (forall<T> s: Seq T, n: int, k: int ::
+axiom {:root} (forall<T> s: Seq T, n: int, k: int ::
   {:weight 25}
   { Seq#Index(s, k), Seq#Drop(s,n) }
   0 <= n && n <= k && k < Seq#Length(s) ==>
     Seq#Index(Seq#Drop(s,n), k-n) == Seq#Index(s, k));
 
-axiom (forall<T> s, t: Seq T, n: int ::
+axiom {:root} (forall<T> s, t: Seq T, n: int ::
   { Seq#Take(Seq#Append(s, t), n) }
   { Seq#Drop(Seq#Append(s, t), n) }
   n == Seq#Length(s)
@@ -1080,10 +1090,10 @@ axiom (forall<T> s, t: Seq T, n: int ::
   Seq#Drop(Seq#Append(s, t), n) == t);
 
 function Seq#FromArray(h: Heap, a: ref): Seq Box;
-axiom (forall h: Heap, a: ref ::
+axiom {:root} (forall h: Heap, a: ref ::
   { Seq#Length(Seq#FromArray(h,a)) }
   Seq#Length(Seq#FromArray(h, a)) == _System.array.Length(a));
-axiom (forall h: Heap, a: ref ::
+axiom {:root} (forall h: Heap, a: ref ::
   { Seq#FromArray(h, a) }
   (forall i: int ::
     // it's important to include both triggers, so that assertions about the
@@ -1095,57 +1105,57 @@ axiom (forall h: Heap, a: ref ::
     i < Seq#Length(Seq#FromArray(h, a))  // this will trigger the previous axiom to get a connection with _System.array.Length(a)
     ==>
     Seq#Index(Seq#FromArray(h, a), i) == read(h, a, IndexField(i))));
-axiom (forall h0, h1: Heap, a: ref ::
+axiom {:root} (forall h0, h1: Heap, a: ref ::
   { Seq#FromArray(h1, a), $HeapSucc(h0, h1) }
   $IsGoodHeap(h0) && $IsGoodHeap(h1) && $HeapSucc(h0, h1) && h0[a] == h1[a]
   ==>
   Seq#FromArray(h0, a) == Seq#FromArray(h1, a));
-axiom (forall h: Heap, i: int, v: Box, a: ref ::
+axiom {:root} (forall h: Heap, i: int, v: Box, a: ref ::
   { Seq#FromArray(update(h, a, IndexField(i), v), a) }
     0 <= i && i < _System.array.Length(a) ==> Seq#FromArray(update(h, a, IndexField(i), v), a) == Seq#Update(Seq#FromArray(h, a), i, v) );
 
 // Commutability of Take and Drop with Update.
-axiom (forall<T> s: Seq T, i: int, v: T, n: int ::
+axiom {:root} (forall<T> s: Seq T, i: int, v: T, n: int ::
         { Seq#Take(Seq#Update(s, i, v), n) }
         0 <= i && i < n && n <= Seq#Length(s) ==> Seq#Take(Seq#Update(s, i, v), n) == Seq#Update(Seq#Take(s, n), i, v) );
-axiom (forall<T> s: Seq T, i: int, v: T, n: int ::
+axiom {:root} (forall<T> s: Seq T, i: int, v: T, n: int ::
         { Seq#Take(Seq#Update(s, i, v), n) }
         n <= i && i < Seq#Length(s) ==> Seq#Take(Seq#Update(s, i, v), n) == Seq#Take(s, n));
-axiom (forall<T> s: Seq T, i: int, v: T, n: int ::
+axiom {:root} (forall<T> s: Seq T, i: int, v: T, n: int ::
         { Seq#Drop(Seq#Update(s, i, v), n) }
         0 <= n && n <= i && i < Seq#Length(s) ==> Seq#Drop(Seq#Update(s, i, v), n) == Seq#Update(Seq#Drop(s, n), i-n, v) );
-axiom (forall<T> s: Seq T, i: int, v: T, n: int ::
+axiom {:root} (forall<T> s: Seq T, i: int, v: T, n: int ::
         { Seq#Drop(Seq#Update(s, i, v), n) }
         0 <= i && i < n && n < Seq#Length(s) ==> Seq#Drop(Seq#Update(s, i, v), n) == Seq#Drop(s, n));
 // Extension axiom, triggers only on Takes from arrays.
-axiom (forall h: Heap, a: ref, n0, n1: int ::
+axiom {:root} (forall h: Heap, a: ref, n0, n1: int ::
         { Seq#Take(Seq#FromArray(h, a), n0), Seq#Take(Seq#FromArray(h, a), n1) }
         n0 + 1 == n1 && 0 <= n0 && n1 <= _System.array.Length(a) ==> Seq#Take(Seq#FromArray(h, a), n1) == Seq#Build(Seq#Take(Seq#FromArray(h, a), n0), read(h, a, IndexField(n0): Field Box)) );
 // drop commutes with build.
-axiom (forall<T> s: Seq T, v: T, n: int ::
+axiom {:root} (forall<T> s: Seq T, v: T, n: int ::
         { Seq#Drop(Seq#Build(s, v), n) }
         0 <= n && n <= Seq#Length(s) ==> Seq#Drop(Seq#Build(s, v), n) == Seq#Build(Seq#Drop(s, n), v) );
 
 function Seq#Rank<T>(Seq T): int;
-axiom (forall s: Seq Box, i: int ::
+axiom {:root} (forall s: Seq Box, i: int ::
         { DtRank($Unbox(Seq#Index(s, i)): DatatypeType) }
         0 <= i && i < Seq#Length(s) ==> DtRank($Unbox(Seq#Index(s, i)): DatatypeType) < Seq#Rank(s) );
-axiom (forall<T> s: Seq T, i: int ::
+axiom {:root} (forall<T> s: Seq T, i: int ::
         { Seq#Rank(Seq#Drop(s, i)) }
         0 < i && i <= Seq#Length(s) ==> Seq#Rank(Seq#Drop(s, i)) < Seq#Rank(s) );
-axiom (forall<T> s: Seq T, i: int ::
+axiom {:root} (forall<T> s: Seq T, i: int ::
         { Seq#Rank(Seq#Take(s, i)) }
         0 <= i && i < Seq#Length(s) ==> Seq#Rank(Seq#Take(s, i)) < Seq#Rank(s) );
-axiom (forall<T> s: Seq T, i: int, j: int ::
+axiom {:root} (forall<T> s: Seq T, i: int, j: int ::
         { Seq#Rank(Seq#Append(Seq#Take(s, i), Seq#Drop(s, j))) }
         0 <= i && i < j && j <= Seq#Length(s) ==> Seq#Rank(Seq#Append(Seq#Take(s, i), Seq#Drop(s, j))) < Seq#Rank(s) );
 
 // Additional axioms about common things
-axiom (forall<T> s: Seq T, n: int :: { Seq#Drop(s, n) }
+axiom {:root} (forall<T> s: Seq T, n: int :: { Seq#Drop(s, n) }
         n == 0 ==> Seq#Drop(s, n) == s);
-axiom (forall<T> s: Seq T, n: int :: { Seq#Take(s, n) }
+axiom {:root} (forall<T> s: Seq T, n: int :: { Seq#Take(s, n) }
         n == 0 ==> Seq#Take(s, n) == Seq#Empty());
-axiom (forall<T> s: Seq T, m, n: int :: { Seq#Drop(Seq#Drop(s, m), n) }
+axiom {:root} (forall<T> s: Seq T, m, n: int :: { Seq#Drop(Seq#Drop(s, m), n) }
         0 <= m && 0 <= n && m+n <= Seq#Length(s) ==>
         Seq#Drop(Seq#Drop(s, m), n) == Seq#Drop(s, m+n));
 
@@ -1163,29 +1173,29 @@ function Map#Elements<U,V>(Map U V) : [U]V;
 
 function Map#Card<U,V>(Map U V) : int;
 
-axiom (forall<U,V> m: Map U V :: { Map#Card(m) } 0 <= Map#Card(m));
+axiom {:root} (forall<U,V> m: Map U V :: { Map#Card(m) } 0 <= Map#Card(m));
 
-axiom (forall<U, V> m: Map U V ::
+axiom {:root} (forall<U, V> m: Map U V ::
   { Map#Card(m) }
   Map#Card(m) == 0 <==> m == Map#Empty());
 
-axiom (forall<U, V> m: Map U V ::
+axiom {:root} (forall<U, V> m: Map U V ::
   { Map#Domain(m) }
   m == Map#Empty() || (exists k: U :: Map#Domain(m)[k]));
-axiom (forall<U, V> m: Map U V ::
+axiom {:root} (forall<U, V> m: Map U V ::
   { Map#Values(m) }
   m == Map#Empty() || (exists v: V :: Map#Values(m)[v]));
-axiom (forall<U, V> m: Map U V ::
+axiom {:root} (forall<U, V> m: Map U V ::
   { Map#Items(m) }
   m == Map#Empty() || (exists k, v: Box :: Map#Items(m)[$Box(#_System._tuple#2._#Make2(k, v))]));
 
-axiom (forall<U, V> m: Map U V ::
+axiom {:root} (forall<U, V> m: Map U V ::
   { Set#Card(Map#Domain(m)) }
   Set#Card(Map#Domain(m)) == Map#Card(m));
-axiom (forall<U, V> m: Map U V ::
+axiom {:root} (forall<U, V> m: Map U V ::
   { Set#Card(Map#Values(m)) }
   Set#Card(Map#Values(m)) <= Map#Card(m));
-axiom (forall<U, V> m: Map U V ::
+axiom {:root} (forall<U, V> m: Map U V ::
   { Set#Card(Map#Items(m)) }
   Set#Card(Map#Items(m)) == Map#Card(m));
 
@@ -1196,7 +1206,7 @@ axiom (forall<U, V> m: Map U V ::
 
 function Map#Values<U,V>(Map U V) : Set V;
 
-axiom (forall<U,V> m: Map U V, v: V :: { Map#Values(m)[v] }
+axiom {:root} (forall<U,V> m: Map U V, v: V :: { Map#Values(m)[v] }
   Map#Values(m)[v] ==
 	(exists u: U :: { Map#Domain(m)[u] } { Map#Elements(m)[u] }
 	  Map#Domain(m)[u] &&
@@ -1217,7 +1227,7 @@ function #_System._tuple#2._#Make2(Box, Box) : DatatypeType;
 function _System.Tuple2._0(DatatypeType) : Box;
 function _System.Tuple2._1(DatatypeType) : Box;
 
-axiom (forall m: Map Box Box, item: Box :: { Map#Items(m)[item] }
+axiom {:root} (forall m: Map Box Box, item: Box :: { Map#Items(m)[item] }
   Map#Items(m)[item] <==>
     Map#Domain(m)[_System.Tuple2._0($Unbox(item))] &&
     Map#Elements(m)[_System.Tuple2._0($Unbox(item))] == _System.Tuple2._1($Unbox(item)));
@@ -1225,18 +1235,18 @@ axiom (forall m: Map Box Box, item: Box :: { Map#Items(m)[item] }
 // Here are the operations that produce Map values.
 
 function Map#Empty<U, V>(): Map U V;
-axiom (forall<U, V> u: U ::
+axiom {:root} (forall<U, V> u: U ::
         { Map#Domain(Map#Empty(): Map U V)[u] }
         !Map#Domain(Map#Empty(): Map U V)[u]);
 
 function Map#Glue<U, V>([U]bool, [U]V, Ty): Map U V;
-axiom (forall<U, V> a: [U]bool, b: [U]V, t: Ty ::
+axiom {:root} (forall<U, V> a: [U]bool, b: [U]V, t: Ty ::
   { Map#Domain(Map#Glue(a, b, t)) }
   Map#Domain(Map#Glue(a, b, t)) == a);
-axiom (forall<U, V> a: [U]bool, b: [U]V, t: Ty ::
+axiom {:root} (forall<U, V> a: [U]bool, b: [U]V, t: Ty ::
   { Map#Elements(Map#Glue(a, b, t)) }
   Map#Elements(Map#Glue(a, b, t)) == b);
-axiom (forall a: [Box]bool, b: [Box]Box, t0, t1: Ty ::
+axiom {:root} (forall a: [Box]bool, b: [Box]Box, t0, t1: Ty ::
   { Map#Glue(a, b, TMap(t0, t1)) }
   // In the following line, no trigger needed, since the quantifier only gets used in negative contexts
   (forall bx: Box :: a[bx] ==> $IsBox(bx, t0) && $IsBox(b[bx], t1))
@@ -1250,50 +1260,50 @@ function Map#Build<U, V>(Map U V, U, V): Map U V;
   { Map#Domain(Map#Build(m, u, v))[u] } { Map#Elements(Map#Build(m, u, v))[u] }
   Map#Domain(Map#Build(m, u, v))[u] && Map#Elements(Map#Build(m, u, v))[u] == v);*/
 
-axiom (forall<U, V> m: Map U V, u: U, u': U, v: V ::
+axiom {:root} (forall<U, V> m: Map U V, u: U, u': U, v: V ::
   { Map#Domain(Map#Build(m, u, v))[u'] } { Map#Elements(Map#Build(m, u, v))[u'] }
   (u' == u ==> Map#Domain(Map#Build(m, u, v))[u'] &&
                Map#Elements(Map#Build(m, u, v))[u'] == v) &&
   (u' != u ==> Map#Domain(Map#Build(m, u, v))[u'] == Map#Domain(m)[u'] &&
                Map#Elements(Map#Build(m, u, v))[u'] == Map#Elements(m)[u']));
-axiom (forall<U, V> m: Map U V, u: U, v: V :: { Map#Card(Map#Build(m, u, v)) }
+axiom {:root} (forall<U, V> m: Map U V, u: U, v: V :: { Map#Card(Map#Build(m, u, v)) }
   Map#Domain(m)[u] ==> Map#Card(Map#Build(m, u, v)) == Map#Card(m));
-axiom (forall<U, V> m: Map U V, u: U, v: V :: { Map#Card(Map#Build(m, u, v)) }
+axiom {:root} (forall<U, V> m: Map U V, u: U, v: V :: { Map#Card(Map#Build(m, u, v)) }
   !Map#Domain(m)[u] ==> Map#Card(Map#Build(m, u, v)) == Map#Card(m) + 1);
 
 // Map operations
 function Map#Merge<U, V>(Map U V, Map U V): Map U V;
-axiom (forall<U, V> m: Map U V, n: Map U V ::
+axiom {:root} (forall<U, V> m: Map U V, n: Map U V ::
   { Map#Domain(Map#Merge(m, n)) }
   Map#Domain(Map#Merge(m, n)) == Set#Union(Map#Domain(m), Map#Domain(n)));
-axiom (forall<U, V> m: Map U V, n: Map U V, u: U ::
+axiom {:root} (forall<U, V> m: Map U V, n: Map U V, u: U ::
   { Map#Elements(Map#Merge(m, n))[u] }
   Map#Domain(Map#Merge(m, n))[u] ==>
     (!Map#Domain(n)[u] ==> Map#Elements(Map#Merge(m, n))[u] == Map#Elements(m)[u]) &&
     (Map#Domain(n)[u] ==> Map#Elements(Map#Merge(m, n))[u] == Map#Elements(n)[u]));
 
 function Map#Subtract<U, V>(Map U V, Set U): Map U V;
-axiom (forall<U, V> m: Map U V, s: Set U ::
+axiom {:root} (forall<U, V> m: Map U V, s: Set U ::
   { Map#Domain(Map#Subtract(m, s)) }
   Map#Domain(Map#Subtract(m, s)) == Set#Difference(Map#Domain(m), s));
-axiom (forall<U, V> m: Map U V, s: Set U, u: U ::
+axiom {:root} (forall<U, V> m: Map U V, s: Set U, u: U ::
   { Map#Elements(Map#Subtract(m, s))[u] }
   Map#Domain(Map#Subtract(m, s))[u] ==>
     Map#Elements(Map#Subtract(m, s))[u] == Map#Elements(m)[u]);
 
 //equality for maps
 function Map#Equal<U, V>(Map U V, Map U V): bool;
-axiom (forall<U, V> m: Map U V, m': Map U V::
+axiom {:root} (forall<U, V> m: Map U V, m': Map U V::
   { Map#Equal(m, m') }
     Map#Equal(m, m') <==> (forall u : U :: Map#Domain(m)[u] == Map#Domain(m')[u]) &&
                           (forall u : U :: Map#Domain(m)[u] ==> Map#Elements(m)[u] == Map#Elements(m')[u]));
 // extensionality
-axiom (forall<U, V> m: Map U V, m': Map U V::
+axiom {:root} (forall<U, V> m: Map U V, m': Map U V::
   { Map#Equal(m, m') }
     Map#Equal(m, m') ==> m == m');
 
 function Map#Disjoint<U, V>(Map U V, Map U V): bool;
-axiom (forall<U, V> m: Map U V, m': Map U V ::
+axiom {:root} (forall<U, V> m: Map U V, m': Map U V ::
   { Map#Disjoint(m, m') }
     Map#Disjoint(m, m') <==> (forall o: U :: {Map#Domain(m)[o]} {Map#Domain(m')[o]} !Map#Domain(m)[o] || !Map#Domain(m')[o]));
 
@@ -1309,23 +1319,23 @@ function IMap#Domain<U,V>(IMap U V) : Set U;
 
 function IMap#Elements<U,V>(IMap U V) : [U]V;
 
-axiom (forall<U, V> m: IMap U V ::
+axiom {:root} (forall<U, V> m: IMap U V ::
   { IMap#Domain(m) }
   m == IMap#Empty() || (exists k: U :: IMap#Domain(m)[k]));
-axiom (forall<U, V> m: IMap U V ::
+axiom {:root} (forall<U, V> m: IMap U V ::
   { IMap#Values(m) }
   m == IMap#Empty() || (exists v: V :: IMap#Values(m)[v]));
-axiom (forall<U, V> m: IMap U V ::
+axiom {:root} (forall<U, V> m: IMap U V ::
   { IMap#Items(m) }
   m == IMap#Empty() || (exists k, v: Box :: IMap#Items(m)[$Box(#_System._tuple#2._#Make2(k, v))]));
 
-axiom (forall<U, V> m: IMap U V ::
+axiom {:root} (forall<U, V> m: IMap U V ::
   { IMap#Domain(m) }
   m == IMap#Empty() <==> IMap#Domain(m) == ISet#Empty());
-axiom (forall<U, V> m: IMap U V ::
+axiom {:root} (forall<U, V> m: IMap U V ::
   { IMap#Values(m) }
   m == IMap#Empty() <==> IMap#Values(m) == ISet#Empty());
-axiom (forall<U, V> m: IMap U V ::
+axiom {:root} (forall<U, V> m: IMap U V ::
   { IMap#Items(m) }
   m == IMap#Empty() <==> IMap#Items(m) == ISet#Empty());
 
@@ -1336,7 +1346,7 @@ axiom (forall<U, V> m: IMap U V ::
 
 function IMap#Values<U,V>(IMap U V) : Set V;
 
-axiom (forall<U,V> m: IMap U V, v: V :: { IMap#Values(m)[v] }
+axiom {:root} (forall<U,V> m: IMap U V, v: V :: { IMap#Values(m)[v] }
   IMap#Values(m)[v] ==
 	(exists u: U :: { IMap#Domain(m)[u] } { IMap#Elements(m)[u] }
 	  IMap#Domain(m)[u] &&
@@ -1353,25 +1363,25 @@ axiom (forall<U,V> m: IMap U V, v: V :: { IMap#Values(m)[v] }
 
 function IMap#Items<U,V>(IMap U V) : Set Box;
 
-axiom (forall m: IMap Box Box, item: Box :: { IMap#Items(m)[item] }
+axiom {:root} (forall m: IMap Box Box, item: Box :: { IMap#Items(m)[item] }
   IMap#Items(m)[item] <==>
     IMap#Domain(m)[_System.Tuple2._0($Unbox(item))] &&
     IMap#Elements(m)[_System.Tuple2._0($Unbox(item))] == _System.Tuple2._1($Unbox(item)));
 
 // Here are the operations that produce Map values.
 function IMap#Empty<U, V>(): IMap U V;
-axiom (forall<U, V> u: U ::
+axiom {:root} (forall<U, V> u: U ::
         { IMap#Domain(IMap#Empty(): IMap U V)[u] }
         !IMap#Domain(IMap#Empty(): IMap U V)[u]);
 
 function IMap#Glue<U, V>([U] bool, [U]V, Ty): IMap U V;
-axiom (forall<U, V> a: [U]bool, b: [U]V, t: Ty ::
+axiom {:root} (forall<U, V> a: [U]bool, b: [U]V, t: Ty ::
   { IMap#Domain(IMap#Glue(a, b, t)) }
   IMap#Domain(IMap#Glue(a, b, t)) == a);
-axiom (forall<U, V> a: [U]bool, b: [U]V, t: Ty ::
+axiom {:root} (forall<U, V> a: [U]bool, b: [U]V, t: Ty ::
   { IMap#Elements(IMap#Glue(a, b, t)) }
   IMap#Elements(IMap#Glue(a, b, t)) == b);
-axiom (forall a: [Box]bool, b: [Box]Box, t0, t1: Ty ::
+axiom {:root} (forall a: [Box]bool, b: [Box]Box, t0, t1: Ty ::
   { IMap#Glue(a, b, TIMap(t0, t1)) }
   // In the following line, no trigger needed, since the quantifier only gets used in negative contexts
   (forall bx: Box :: a[bx] ==> $IsBox(bx, t0) && $IsBox(b[bx], t1))
@@ -1384,7 +1394,7 @@ function IMap#Build<U, V>(IMap U V, U, V): IMap U V;
   { IMap#Domain(IMap#Build(m, u, v))[u] } { IMap#Elements(IMap#Build(m, u, v))[u] }
   IMap#Domain(IMap#Build(m, u, v))[u] && IMap#Elements(IMap#Build(m, u, v))[u] == v);*/
 
-axiom (forall<U, V> m: IMap U V, u: U, u': U, v: V ::
+axiom {:root} (forall<U, V> m: IMap U V, u: U, u': U, v: V ::
   { IMap#Domain(IMap#Build(m, u, v))[u'] } { IMap#Elements(IMap#Build(m, u, v))[u'] }
   (u' == u ==> IMap#Domain(IMap#Build(m, u, v))[u'] &&
                IMap#Elements(IMap#Build(m, u, v))[u'] == v) &&
@@ -1393,31 +1403,31 @@ axiom (forall<U, V> m: IMap U V, u: U, u': U, v: V ::
 
 //equality for imaps
 function IMap#Equal<U, V>(IMap U V, IMap U V): bool;
-axiom (forall<U, V> m: IMap U V, m': IMap U V::
+axiom {:root} (forall<U, V> m: IMap U V, m': IMap U V::
   { IMap#Equal(m, m') }
     IMap#Equal(m, m') <==> (forall u : U :: IMap#Domain(m)[u] == IMap#Domain(m')[u]) &&
                           (forall u : U :: IMap#Domain(m)[u] ==> IMap#Elements(m)[u] == IMap#Elements(m')[u]));
 // extensionality
-axiom (forall<U, V> m: IMap U V, m': IMap U V::
+axiom {:root} (forall<U, V> m: IMap U V, m': IMap U V::
   { IMap#Equal(m, m') }
     IMap#Equal(m, m') ==> m == m');
 
 // IMap operations
 function IMap#Merge<U, V>(IMap U V, IMap U V): IMap U V;
-axiom (forall<U, V> m: IMap U V, n: IMap U V ::
+axiom {:root} (forall<U, V> m: IMap U V, n: IMap U V ::
   { IMap#Domain(IMap#Merge(m, n)) }
   IMap#Domain(IMap#Merge(m, n)) == Set#Union(IMap#Domain(m), IMap#Domain(n)));
-axiom (forall<U, V> m: IMap U V, n: IMap U V, u: U ::
+axiom {:root} (forall<U, V> m: IMap U V, n: IMap U V, u: U ::
   { IMap#Elements(IMap#Merge(m, n))[u] }
   IMap#Domain(IMap#Merge(m, n))[u] ==>
     (!IMap#Domain(n)[u] ==> IMap#Elements(IMap#Merge(m, n))[u] == IMap#Elements(m)[u]) &&
     (IMap#Domain(n)[u] ==> IMap#Elements(IMap#Merge(m, n))[u] == IMap#Elements(n)[u]));
 
 function IMap#Subtract<U, V>(IMap U V, Set U): IMap U V;
-axiom (forall<U, V> m: IMap U V, s: Set U ::
+axiom {:root} (forall<U, V> m: IMap U V, s: Set U ::
   { IMap#Domain(IMap#Subtract(m, s)) }
   IMap#Domain(IMap#Subtract(m, s)) == Set#Difference(IMap#Domain(m), s));
-axiom (forall<U, V> m: IMap U V, s: Set U, u: U ::
+axiom {:root} (forall<U, V> m: IMap U V, s: Set U, u: U ::
   { IMap#Elements(IMap#Subtract(m, s))[u] }
   IMap#Domain(IMap#Subtract(m, s))[u] ==>
     IMap#Elements(IMap#Subtract(m, s))[u] == IMap#Elements(m)[u]);
@@ -1443,10 +1453,10 @@ function Add(x, y: int): int { x + y }
 function Sub(x, y: int): int { x - y }
 
 #if ARITH_DISTR
-axiom (forall x, y, z: int ::
+axiom {:root} (forall x, y, z: int ::
   { Mul(Add(x, y), z) }
   Mul(Add(x, y), z) == Add(Mul(x, z), Mul(y, z)));
-axiom (forall x,y,z: int ::
+axiom {:root} (forall x,y,z: int ::
   { Mul(x, Add(y, z)) }
   Mul(x, Add(y, z)) == Add(Mul(x, y), Mul(x, z)));
 //axiom (forall x, y, z: int ::
@@ -1454,24 +1464,24 @@ axiom (forall x,y,z: int ::
 //  Mul(Sub(x, y), z) == Sub(Mul(x, z), Mul(y, z)));
 #endif
 #if ARITH_MUL_DIV_MOD
-axiom (forall x, y: int ::
+axiom {:root} (forall x, y: int ::
   { Div(x, y), Mod(x, y) }
   { Mul(Div(x, y), y) }
   y != 0 ==>
   Mul(Div(x, y), y) + Mod(x, y) == x);
 #endif
 #if ARITH_MUL_SIGN
-axiom (forall x, y: int ::
+axiom {:root} (forall x, y: int ::
   { Mul(x, y) }
   ((0 <= x && 0 <= y) || (x <= 0 && y <= 0) ==> 0 <= Mul(x, y)));
 #endif
 #if ARITH_MUL_COMM
-axiom (forall x, y: int ::
+axiom {:root} (forall x, y: int ::
   { Mul(x, y) }
   Mul(x, y) == Mul(y, x));
 #endif
 #if ARITH_MUL_ASSOC
-axiom (forall x, y, z: int ::
+axiom {:root} (forall x, y, z: int ::
   { Mul(x, Mul(y, z)) }
   Mul(y, z) != z && Mul(y, z) != y ==> Mul(x, Mul(y, z)) == Mul(Mul(x, y), z));
 #endif
